theories/overlap.v
@@ -24,3 +24,72 @@ Proof.
   { split; intro; etrans; done. }
   eapply overlap_mono; eauto.
 Qed.
+
+Definition merge_along_loop `{FinMap A M} {B} (m: M B) k (m': M B) :=
+  match m!!k with Some v => <[k:=v]>m' | None => delete k m' end.
+
+Definition merge_along `{FinCollection A C, FinMap A M} {B} (s: C) (m m': M B) :=
+  collection_fold (merge_along_loop m) m' s.
+Infix "~[ s ]~>" := (merge_along s) (at level 50).
+
+Section Facts.
+  Context `{FinCollection A C, FinMap A M}.
+  Instance elem_of_dec_C (x: A) (s: C): Decision (x ∈ s) := elem_of_dec_slow x s.
+
+  Lemma merge_along_cases
+        {B} (s: C) (m m': M B) (k: A):
+    (m ~[s]~> m')!!k = if bool_decide (k ∈ s) then m!!k else m'!!k.
+  Proof.
+    unfold merge_along.
+    refine (collection_fold_ind
+              (λ m'' s'', m''!!k = if bool_decide (k ∈ s'') then m!!k else m'!!k)
+              (merge_along_loop m)
+              m' _ _ _ s);
+      try done.
+    - intros m'' ? <- s' s'' eqs.
+      rewrite (bool_decide_iff (k ∈ s') (k ∈ s'')); auto.
+    - rewrite bool_decide_false; auto.
+      set_solver.
+    - intros k' s' m'' notin IH.
+      unfold merge_along_loop.
+      destruct (decide (k = k')) as [<-|neq].
+      + destruct (m!!k).
+        * by rewrite lookup_insert, bool_decide_true by set_solver.
+        * by rewrite lookup_delete, bool_decide_true by set_solver.
+      + rewrite <-(bool_decide_iff (k ∈ s') (k ∈ {[k']} ∪ s')) by set_solver.
+        rewrite <- IH.
+        destruct (m!!k').
+        * by rewrite lookup_insert_ne.
+        * by rewrite lookup_delete_ne.
+  Qed.
+
+  Lemma lookup_merge_along_in {B} (s: C) (m m': M B) (k: A) (ink: k ∈ s):
+    (m ~[s]~> m')!!k = m!!k.
+  Proof. by rewrite merge_along_cases, bool_decide_true. Qed.
+  Lemma lookup_merge_along_not_in {B} (s: C) (m m': M B) (k: A) (ink: k ∉ s):
+    (m ~[s]~> m')!!k = m'!!k.
+  Proof. by rewrite merge_along_cases, bool_decide_false. Qed.
+
+  Lemma overlap_merge_along_l {B} (s: C) (m m': M B):
+    (m ~[s]~> m') ≡[ s ]≡ m.
+  Proof.
+    intros k ink.
+    rewrite lookup_merge_along_in; done.
+  Qed.
+
+  Lemma overlap_merge_along_r {B} (s s': C) (disj: s ⊥ s') (m m': M B):
+    (m ~[s]~> m') ≡[ s' ]≡ m'.
+  Proof.
+    intros k ink.
+    rewrite lookup_merge_along_not_in; auto.
+    set_solver.
+  Qed.
+End Facts.
+
+Lemma overlap_cast (s: gset positive) {B} (N N': gmap positive B):
+  N ≡[s]≡ N' ↔ N ≡[of_gset s]≡ N'.
+Proof.
+  unfold overlap.
+  setoid_rewrite elem_of_of_gset.
+  done.
+Qed.
