theories/typetranslation.v
@@ -4,414 +4,439 @@ From iris.algebra Require Import updates agree big_op.
 From esop Require Import types oneshot specification corecalculus overlap.
 From stdpp Require Import gmap coPset.
 
-Module TypeTranslation(AxSem: AxiomaticSemantics).
-  Module Import Axiomatics := AxSem <+ AxiomaticFacts.
-  Variant name_entry := Loc (l: loc) | Task (t: tid) (γ: gname).
-  Definition name_map := gmap gname name_entry.
-  Variant conn_name := RET | name (ξ: gname) | var (x: string).
-  Instance: EqDecision conn_name.
-  Proof. solve_decision. Defined.
-  Instance: Countable conn_name :=
-    Build_Countable conn_name _
-      (λ c, match c with RET => 1 | name ξ => ξ~0 | var x => (encode x)~1 end)%positive
-      (λ p, match p with 1 => Some RET | ξ~0 => Some (name ξ) | x~1 => var <$> decode x end)%positive
-      _.
+Variant name_entry := Loc (l: loc) | Task (t: tid) (γ: gname).
+Definition name_map := gmap gname name_entry.
+Variant conn_name := RET | name (ξ: gname) | var (x: string).
+Instance: EqDecision conn_name.
+Proof. solve_decision. Defined.
+Definition conn_name_encode c :=
+  (match c with RET => 1 | name ξ => ξ~0 | var x => (encode x)~1 end)%positive.
+Definition conn_name_decode p :=
+  (match p with 1 => Some RET | ξ~0 => Some (name ξ) | x~1 => var <$> decode x end)%positive.
+Instance: Countable conn_name :=
+  Build_Countable conn_name _ conn_name_encode conn_name_decode _.
+Proof.
+  destruct x; auto.
+  rewrite /conn_name_encode /conn_name_decode decode_encode; done.
+Qed.
+
+Definition conn_map := gmap conn_name val.
+Definition int_type {Σ} := val → name_map → val → iProp Σ.
+Definition int_heap {Σ} := conn_map → name_map → iProp Σ.
+
+Definition names_heap (η: types.heap): gset conn_name := of_list (name <$> (elements (names η))).
+Lemma elem_of_names_heap (d: conn_name) η:
+  (d ∈ names_heap η ↔ ∃ ξ: gname, d = name ξ ∧ ξ ∈ names η)%type.
+Proof.
+  rewrite /names_heap elem_of_of_list elem_of_list_fmap.
+  f_equiv; intro ξ. by rewrite elem_of_elements.
+Qed.
+
+Definition names_env (Γ: env): gset conn_name := of_list (var <$> fst <$> map_to_list Γ).
+Lemma elem_of_names_env n (Γ: env): n ∈ names_env Γ ↔ ∃ x, n = var x ∧ is_Some (Γ !! x).
+Proof.
+  rewrite /names_env elem_of_of_list -list_fmap_compose elem_of_list_fmap.
+  split.
+  { intros [[x τ] [-> isin%elem_of_map_to_list]].
+    eauto.
+  } {
+    intros [x [-> [τ isin%elem_of_map_to_list]]].
+    exists (x,τ); auto.
+  }
+Qed.
+Lemma env_elem_of_names ξ (Γ: env): ξ ∈ names Γ ↔ ∃ x τ, Γ !! x = Some τ ∧ ξ ∈ names τ.
+Proof.
+  rewrite {1}/names /Names_instance_2.
+  induction Γ as [|x τ] using map_ind.
+  { rewrite big_opM_empty elem_of_empty.
+    setoid_rewrite lookup_empty.
+    firstorder. }
+  rewrite big_opM_insert; last done.
+  rewrite elem_of_union IHΓ.
+  split.
+  { intros [inξ|[x' [τ' [lookup inξ]]]].
+    - exists x, τ.
+      rewrite lookup_insert; auto.
+    - exists x', τ'.
+      rewrite lookup_insert_ne; auto.
+      intros <-.
+      rewrite H in lookup; discriminate. }
+  intros [x' [τ' [mt inξ]]].
+  destruct (decide (x=x')) as [<-|neq].
+  { rewrite lookup_insert in mt.
+    injection mt as <-; auto. }
+  rewrite lookup_insert_ne in mt; last done.
+  eauto.
+Qed.
+
+Record task_data :=
+  TaskData {
+      td_expr: expr;
+      td_env: env;
+      td_pre: types.heap;
+      td_post: types.heap;
+      td_alloc: gset gname;
+      td_D_pre: conn_map;
+      td_D_name: gname;
+      td_N_name: gname
+    }.
+Canonical Structure task_dataC := leibnizC task_data.
+Canonical Structure conn_mapC := leibnizC conn_map.
+Canonical Structure name_mapC := leibnizC name_map.
+Class taskDataG Σ :=
+  { td_taskData_inG:> inG Σ (agreeR task_dataC);
+    td_connData_inG:> inG Σ (oneshotR conn_mapC);
+    td_nameData_inG:> inG Σ (oneshotR name_mapC) }.
+Local Open Scope I.
+
+Definition intΓ {Σ} (iτ: type → int_type) (Γ: env) (D: conn_map) (N: name_map)
+           (σ: gmap string val): iProp Σ :=
+  ⌜(∀ x: string, is_Some (Γ !! x) ↔ is_Some (σ !! x)) ∧
+   (∀ x: string, is_Some (Γ !! x) → is_Some (D !! var x))⌝ ∧
+  ∀ (x: string) τ v d, ⌜Γ !! x = Some τ ∧
+                       σ !! x = Some v ∧
+                       D !! var x = Some d⌝ → iτ τ d N v.
+
+Definition not_new A: coPset := ⊤ ∖ of_gset A.
+Class InitialConfiguration := initial_cfg: cfg.
+Class WaitPermissions :=
+  { wp_axiomaticIrisG: gFunctors → Set;
+    wp_axiomatic_implies_inv :> ∀ `{wp_axiomaticIrisG Σ}, invG Σ;
+    wp_wait: ∀ `{wp_axiomaticIrisG Σ}, tid → (val → iProp Σ) → iProp Σ }.
+Existing Class wp_axiomaticIrisG.
+
+Definition simulation_body `{specStateG Σ, invG Σ, inG Σ heapR,InitialConfiguration}
+           iτ (iη: types.heap → int_heap) Γ e η A τ η' D D': iProp Σ :=
+  ∀ N σ, existential_triple ⊤ initial_cfg
+                            (intΓ iτ Γ D N σ ∗ iη η D N)
+                            (subst (of_val <$> σ) e)
+                            (λ v, ∃ d N',
+                                ⌜N ≡[not_new A]≡ N' ∧ D' !! RET = Some d⌝ ∧
+                                iτ τ d N' v ∗ iη η' D' N').
+
+Section TypeInterpretation.
+  Context `{WaitPermissions, implStateG Σ, specStateG Σ, taskDataG Σ}.
+  Context `{wp_axiomaticIrisG _ Σ,InitialConfiguration}.
+  Implicit Type d : val.
+  Implicit Type N: name_map.
+  Implicit Type x: val.
+
+  Definition int_i_bool d N x: iProp Σ := ⌜(x = Ctrue ∨ x = Cfalse) ∧ x = d⌝.
+  Definition int_s_bool := int_i_bool.
+  Definition int_i_unit d N x: iProp Σ := ⌜x = Cunit⌝.
+  Definition int_s_unit := int_i_unit.
+  Definition int_i_ref (ξ: gname) d N x: iProp Σ := ⌜∃ l: loc, N!!ξ = Some (Loc l) ∧ x = Cloc l⌝.
+  Definition int_s_ref := int_i_ref.
+  Definition int_s_promise ξ d N x: iProp Σ := ⌜∃ t γ, N!!ξ = Some (Task t γ) ∧ x = Ctid t⌝.
+
+  (** We build the implementation interpretation of promise in stages. *)
+  (** Access to the task data. *)
+  Definition ip_data γ U (D': conn_map) (N': name_map) :=
+    own γ (to_agree U) ∗ own (td_D_name U) (agreed D') ∗ own (td_N_name U) (agreed N').
+  (** The easy parts: name map and implementation interpretation. *)
+  Definition ip_impl (A: gset gname) (τ: type) (τi: @int_type Σ) (D': conn_map) N' N y :=
+    ∃ d, ⌜D' !! RET = Some d ∧ N' ≡[ names τ ∖ A ]≡ N⌝ ∗ τi d N' y.
+  Definition ip_sim iτs iηs τ U D' :=
+    simulation_body iτs iηs
+                    (td_env U) (td_expr U) (td_pre U) (td_alloc U) τ (td_post U) (td_D_pre U) D'.
+  (** Put together the inner pieces of the interpretation of promises... *)
+  Definition promiseN := nroot .@ "promise".
+  Definition int_i_promise_body iτs iηs N A τ τi γ v :=
+    ∃ U D' N',
+      ip_data γ U D' N' ∗ ip_impl A τ τi D' N' N v ∗ □ip_sim iτs iηs τ U D'.
+  Definition int_i_promise iτs iηs ξ A τ τi d N x :=
+    ∃ t γ, ⌜N !! ξ = Some (Task t γ) ∧ x = Ctid t⌝ ∧
+           inv promiseN (wp_wait t (int_i_promise_body iτs iηs (delete ξ N) A τ τi γ)).
+End TypeInterpretation.
+
+Section HeapInterpretation.
+  Context `{WaitPermissions, implStateG Σ, specStateG Σ, wp_axiomaticIrisG _ Σ, taskDataG Σ}.
+  Implicit Type N : name_map.
+  Implicit Type D : conn_map.
+  Local Open Scope I.
+
+  Definition int_i_emp D N: iProp Σ := True.
+  Definition int_s_emp := int_i_emp.
+  Definition int_i_star (iη iη': int_heap) D N: iProp Σ := iη D N ∗ iη' D N.
+  Definition int_s_star := int_i_star.
+  Definition int_i_pt ξ (iτ: int_type) D N: iProp Σ :=
+    ∃ l d v, ⌜N!!ξ = Some (Loc l) ∧ D!!name ξ = Some d⌝ ∗ mapstoI l v 1%Qp ∗ iτ d N v.
+  Definition int_s_pt ξ (iτ: int_type) D N: iProp Σ :=
+    ∃ l d v, ⌜N!!ξ = Some (Loc l) ∧ D!!name ξ = Some d⌝ ∗ mapstoS l v 1%Qp ∗ iτ d N v.
+  Definition int_i_wait_body γ (η: types.heap) (iη: int_heap) A N :=
+    ∃ U D' N', ip_data γ U D' N' ∗ ⌜N ≡[ names η ∖ A]≡ N'⌝ ∗ iη D' N'.
+  Definition int_i_wait ξ A η (iη: int_heap) D N: iProp Σ :=
+    ∃ t γ, ⌜N!!ξ = Some (Task t γ)⌝ ∗ wp_wait t (λ _, int_i_wait_body γ η iη A (delete ξ N)).
+  (* Use the lower-level interpretations here *)
+  Definition int_s_wait_pre iτs' (iηs': types.heap → int_heap) U N' σ: iProp Σ :=
+    intΓ iτs' (td_env U) (td_D_pre U) N' σ ∗ iηs' (td_pre U) (td_D_pre U) N'.
+  Definition int_s_wait iτs' iηs' ξ A η D N :=
+    ∃ t γ U N' σ,
+      ⌜N!!ξ = Some (Task t γ) ∧ td_post U = η ∧ N' ≡[names η ∖ A]≡ N⌝ ∧
+      t ⤇ run: (subst (of_val <$> σ) (td_expr U)) ∗ int_s_wait_pre iτs' iηs' U N' σ.
+End HeapInterpretation.
+
+Section Interpretations.
+  Context `{WaitPermissions, implStateG Σ, specStateG Σ, wp_axiomaticIrisG _ Σ, taskDataG Σ}.
+  Context `{InitialConfiguration, ∀ t, Proper (pointwise_relation _ (≡) ==> (≡)) (wp_wait t)}.
+  Implicit Type N: name_map.
+  Implicit Type D: conn_map.
+  Implicit Type x: val.
+  Implicit Type d: val.
+  Local Open Scope I.
+  
+  Fixpoint int_s_type τ: @int_type Σ :=
+    match τ with
+    | tbool => int_s_bool
+    | tunit => int_s_unit
+    | tref ξ => int_s_ref ξ
+    | ttask ξ A τ => int_s_promise ξ
+    end.
+  Fixpoint int_s_heap_approx iη η: @int_heap Σ :=
+    match η with
+    | hemp => int_s_emp
+    | hstar η η' => int_s_star (int_s_heap_approx iη η) (int_s_heap_approx iη η')
+    | hpt ξ τ => int_s_pt ξ (int_s_type τ)
+    | hwait ξ A η => int_s_wait int_s_type iη ξ A η
+    end.
+  Fixpoint int_s_heap_rec n η :=
+    int_s_heap_approx (match n with
+                       | O => λ _ _ _, False%I
+                       | S n => int_s_heap_rec n
+                       end)
+                      η.
+  Definition int_s_heap η: @int_heap Σ := λ D N, ∃ n, int_s_heap_rec n η D N.
+
+  Fixpoint int_i_type τ: @int_type Σ :=
+    match τ with
+    | tbool => int_i_bool
+    | tunit => int_i_unit
+    | tref ξ => int_i_ref ξ
+    | ttask ξ A τ => int_i_promise int_s_type int_s_heap ξ A τ (int_i_type τ)
+    end.
+  Fixpoint int_i_heap η: @int_heap Σ :=
+    match η with
+    | hemp => int_i_emp
+    | hstar η η' => int_i_star (int_i_heap η) (int_i_heap η')
+    | hpt ξ τ => int_i_pt ξ (int_i_type τ)
+    | hwait ξ A η => int_i_wait ξ A η (int_i_heap η)
+    end.
+
+  Definition int_s_env := intΓ int_s_type.
+  Definition int_i_env := intΓ int_i_type.
+  
+  (** Basic properties of interpretation *)
+  Global Instance int_s_type_persistent τ d N v:  PersistentP (int_s_type τ d N v).
+  Proof. destruct τ; apply _. Qed.
+  Global Instance int_i_type_persistent τ d N v:  PersistentP (int_i_type τ d N v).
+  Proof. destruct τ; apply _. Qed.
+  Global Instance int_s_env_persistent Γ D N σ: PersistentP (int_s_env Γ D N σ).
+  Proof. apply _. Qed.
+  Global Instance int_i_env_persistent Γ D N σ: PersistentP (int_i_env Γ D N σ).
+  Proof. apply _. Qed.
+
+  Global Instance int_s_type_local τ:
+    Proper ((=) ==> overlap (names τ) ==> (=) ==> (⊣⊢)) (int_s_type τ).
   Proof.
-    destruct x; auto.
-    rewrite decode_encode; done.
+    induction τ; intros d ? <- N N' eqN x ? <-; cbn; try done.
+    - rewrite /int_s_ref /int_i_ref.
+      rewrite eqN; first done.
+      cbn; set_solver.
+    - rewrite /int_s_promise.
+      rewrite eqN; first done.
+      cbn -[union]; set_solver.
+  Qed.
+
+  Global Instance int_i_type_local τ:
+    Proper ((=) ==> overlap (names τ) ==> (=) ==> (⊣⊢)) (int_i_type τ).
+  Proof.
+    induction τ; intros d ? <- N N' eqN x ? <-; cbn; try done.
+    - rewrite /int_i_ref eqN; first done.
+      cbn; set_solver.
+    - rewrite /int_i_promise /int_i_promise_body /ip_impl.
+      rewrite (eqN ξ); last set_solver.
+      do 21 f_equiv.
+      apply (overlap_iff ((names (ttask ξ A τ)))).
+      + apply union_subseteq_r.
+      + intros ξ' inξ'.
+        destruct (decide (ξ = ξ')) as [<-|neq].
+        * by rewrite !lookup_delete.
+        * rewrite !lookup_delete_ne; auto.
+  Qed.
+
+  Lemma names_heap_star η η': (names_heap (η ⊗ η') ≡ names_heap η ∪ names_heap η')%C.
+  Proof.
+    rewrite /names_heap => ξ.
+    rewrite elem_of_union !elem_of_of_list !elem_of_list_fmap /=.
+    setoid_rewrite elem_of_elements.
+    change (names (hstar η η')) with (names η ∪ names η').
+    setoid_rewrite elem_of_union.
+    split.
+    - intros [? [? [?|?]]]; eauto.
+    - intros [[? [??]]|[? [??]]]; eauto.
   Qed.
   
-  Definition conn_map := gmap conn_name val.
-  Coercion VConst: const >-> val.
-  
-  Definition int_type {Σ} := val → name_map → val → iProp Σ.
-  Definition int_heap {Σ} := conn_map → name_map → iProp Σ.
+  Lemma int_s_heap_approx_local
+        iη (iη_proper: ∀ (η: types.heap),
+               Proper (overlap (names_heap η) ==> overlap (names η) ==> (⊣⊢)) (iη η)) η:
+    Proper (overlap (names_heap η) ==> overlap (names η) ==> (⊣⊢)) (int_s_heap_approx iη η).
+  Proof.
+    induction η; intros D D' eqD N N' eqN; cbn.
+    - done.
+    - rewrite /int_s_star /int_i_star.
+      f_equiv; [apply IHη1|apply IHη2].
+      all: eapply overlap_mono; eauto.
+      all: cbn.
+      1,3: rewrite names_heap_star.
+      all: clear; set_solver.
+    - rewrite /int_s_pt.
+      setoid_rewrite (eqN ξ); last by set_solver.
+      rewrite eqD; cycle 1.
+      { rewrite /names_heap elem_of_of_list elem_of_list_fmap.
+        exists ξ; split; auto.
+        rewrite elem_of_elements; set_solver. }
+      enough (∀ d v, int_s_type τ d N v ⊣⊢ int_s_type τ d N' v) as eqint.
+      { by setoid_rewrite eqint. }
+      intros; apply int_s_type_local; auto.
+      eapply overlap_mono; eauto.
+      set_solver.
+    - rewrite /int_s_wait /=.
+      do 10 f_equiv.
+      rewrite (eqN ξ); last set_solver.
+      do 4 f_equiv.
+      apply (overlap_iff ((names (hwait ξ A η)))); eauto.
+      apply union_subseteq_r.
+  Qed.
 
-  Record task_data :=
-    TaskData {
-        td_expr: expr;
-        td_env: env;
-        td_pre: types.heap;
-        td_post: types.heap;
-        td_D_pre: conn_map;
-        td_D_name: gname;
-        td_N_name: gname
-      }.
-  Canonical Structure task_dataC := leibnizC task_data.
-  Canonical Structure conn_mapC := leibnizC conn_map.
-  Canonical Structure name_mapC := leibnizC name_map.
-  Class taskDataG Σ :=
-    { td_taskData_inG:> inG Σ (agreeR task_dataC);
-      td_connData_inG:> inG Σ (oneshotR conn_mapC);
-      td_nameData_inG:> inG Σ (oneshotR name_mapC) }.
-  
-  (** First, define functions for each case separately. *)
-  Section TypeInterpretation.
-    Context `{implStateG Σ, specStateG Σ, axiomaticIrisG Σ, taskDataG Σ} (c0: cfg).
-
-    Local Open Scope I.
-    Definition intΓ (iτ: type → int_type) (Γ: env) (D: conn_map) (N: name_map)
-               (σ: gmap string val): iProp Σ :=
-      ⌜∀ x: string, is_Some (Γ !! x) ↔ is_Some (σ !! x)⌝ ∧
-            ⌜∀ x: string, is_Some (Γ !! x) → is_Some (D !! var x)⌝ ∧
-                          ∀ (x: string) τ v d, ⌜Γ !! x = Some τ ∧
-                                               σ !! x = Some v ∧
-                                               D !! var x = Some d⌝ → iτ τ d N v.
-    Definition not_new (Γ: env) (η: types.heap) (τ: type) (η': types.heap): coPset :=
-      of_gset (names Γ ∪ names η) ∖ of_gset (names τ ∪ names η').
-
-    Definition simulation' iτ iτ' (iη iη': types.heap → int_heap) Γ e η τ η' D D': iProp Σ :=
-      ∀ N σ, existential_triple ⊤ c0
-                                (intΓ iτ Γ D N σ ∗ iη η D N)
-                                (subst (of_val <$> σ) e)
-                                (λ v, ∃ d N',
-                                    ⌜N ≡[not_new Γ η τ η']≡ N' ∧ D' !! RET = Some d⌝ ∧
-                                    iτ' τ d N' v ∗ iη' η' D' N').
-    
-    Implicit Type d : val.
-    Implicit Type N: name_map.
-    Implicit Type x: val.
-
-    Definition int_i_bool d N x: iProp Σ := ⌜(x = Ctrue ∨ x = Cfalse) ∧ x = d⌝.
-    Definition int_s_bool := int_i_bool.
-    Definition int_i_unit d N x: iProp Σ := ⌜x = Cunit⌝.
-    Definition int_s_unit := int_i_unit.
-    Definition int_i_ref (ξ: gname) d N x: iProp Σ := ⌜∃ l: loc, N!!ξ = Some (Loc l) ∧ x = Cloc l⌝.
-    Definition int_s_ref := int_i_ref.
-    Definition int_s_promise ξ d N x: iProp Σ := ⌜∃ t γ, N!!ξ = Some (Task t γ) ∧ x = Ctid t⌝.
-
-    (** We build the implementation interpretation of promise in stages. *)
-    (** Access to the task data. *)
-    Definition ip_data γ U (D': conn_map) (N': name_map) :=
-      own γ (to_agree U) ∗ own (td_D_name U) (agreed D') ∗ own (td_N_name U) (agreed N').
-    (** The easy parts: name map and implementation interpretation. *)
-    Definition ip_impl (A: gset gname) (τ: type) (τi: @int_type Σ) (D': conn_map) N' N y :=
-      ∃ d, ⌜D' !! RET = Some d ∧ N' ≡[ of_gset (names τ) ∖ of_gset A ]≡ N⌝ ∗ τi d N' y.
-    (** The simuation triple. Note that we have a bit of trouble here: As given in the
-        paper, the construction is not neccesarily well-founded. The complications with
-        the different its and so on are here to allow us to build a well-founded fixpoint
-        later on. *)
-    Definition ip_sim iτs iτs' iηs iηs' τ U D' :=
-      simulation' iτs iτs' iηs iηs' (td_env U) (td_expr U) (td_pre U) τ (td_post U) (td_D_pre U) D'.
-    (** Now, note that we only need to make our fixpoint well-founded for the
-        preconditions: τ is known to be structurally smaller, and the interpretation
-        of types does not recurse into that of heaps, so we can simply use the
-        same-level functions for the postconditions. But the names in the preconditions
-        will never be in allocation sets, so we can treat them as constant - in other
-        words, we can look up the task ids of all the ξ in the precondition! This allows
-        us to write down a description of type depth (i.e., how long a chain of promises
-        it induces). 
-        us to get the levels for those tasks, and formulate an invariant. *)
-    Fixpoint ty_all_tasks (ϕ: gname → iProp Σ) τ :=
-      match τ return iProp Σ with
-      | ttask ξ _ τ => ϕ ξ ∗ ty_all_tasks ϕ τ
-      | tref _ | tunit | tbool => True
-      end.
-    Fixpoint he_all_tasks (ϕ: gname → iProp Σ) η :=
-      match η return iProp Σ with
-      | hwait ξ _ η => ϕ ξ ∗ he_all_tasks ϕ η
-      | hstar η η' => he_all_tasks ϕ η ∗ he_all_tasks ϕ η'
-      | hpt _ _ | hemp => True
-      end.
-    Definition env_all_tasks ϕ (Γ: env) := ∀ (x: string) τ, ⌜Γ !! x = Some τ⌝ → ty_all_tasks ϕ τ.
-    Fixpoint depth N n γ {struct n} :=
-      match n return iProp Σ with
-      | O => False
-      | S n => ∀ γ (U: task_data),
-          own γ (to_agree U) -∗
-                     let ϕ ξ := (∀ p γ, ⌜N !! ξ = Some (Task p γ)⌝ → depth N n γ)
-                     in env_all_tasks ϕ (td_env U) ∗ he_all_tasks ϕ (td_pre U)
-      end.
-    (** Put together the inner pieces of the interpretation of promises... *)
-    Definition promiseN := nroot .@ "promise".
-    Definition int_i_promise_body iτs iτs' iηs iηs' N A τ τi γ v :=
-      ∀ U D' N',
-        ip_data γ U D' N' ∗ ip_impl A τ τi D' N' N v ∗ ip_sim iτs iτs' iηs iηs' τ U D'.
-    Definition int_i_promise iτs iτs' iηs iηs' ξ A τ τi d N x :=
-      ∃ t γ, ⌜N !! ξ = Some (Task t γ) ∧ x = Ctid t⌝ ∧
-           inv promiseN (wait t (int_i_promise_body iτs iτs' iηs iηs' N A τ τi γ)).
-  End TypeInterpretation.
-  Section HeapInterpretation.
-    Context `{implStateG Σ, specStateG Σ, axiomaticIrisG Σ, taskDataG Σ} (c0: cfg).
-    Implicit Type N : name_map.
-    Implicit Type D : conn_map.
-    Local Open Scope I.
-
-    Definition int_i_emp D N: iProp Σ := True.
-    Definition int_s_emp := int_i_emp.
-    Definition int_i_star (iη iη': int_heap) D N: iProp Σ := iη D N ∗ iη' D N.
-    Definition int_s_star := int_i_star.
-    Definition int_i_pt ξ (iτ: int_type) D N: iProp Σ :=
-      ∃ l d v, ⌜N!!ξ = Some (Loc l) ∧ D!!name ξ = Some d⌝ ∗ mapstoI l v 1%Qp ∗ iτ d N v.
-    Definition int_s_pt ξ (iτ: int_type) D N: iProp Σ :=
-      ∃ l d v, ⌜N!!ξ = Some (Loc l) ∧ D!!name ξ = Some d⌝ ∗ mapstoS l v 1%Qp ∗ iτ d N v.
-    Definition int_i_wait_body γ (η: types.heap) (iη: int_heap) A N :=
-      ∃ U D' N', ip_data γ U D' N' ∗ ⌜N ≡[ of_gset (names η) ∖ of_gset A]≡ N'⌝ ∗ iη D' N'.
-    Definition int_i_wait ξ A η (iη: int_heap) D N: iProp Σ :=
-      ∃ t γ, ⌜N!!ξ = Some (Task t γ)⌝ ∗ wait t (λ _, int_i_wait_body γ η iη A N).
-    (* Use the lower-level interpretations here *)
-    Definition int_s_wait_pre iτs' (iηs': types.heap → int_heap) U N' σ: iProp Σ :=
-      intΓ iτs' (td_env U) (td_D_pre U) N' σ ∗ iηs' (td_pre U) (td_D_pre U) N'.
-    Definition int_s_wait iτs' iηs' ξ A η D N :=
-      ∃ t γ U N' σ,
-        ⌜N!!ξ = Some (Task t γ) ∧ td_post U = η ∧ N' ≡[of_gset (names η) ∖ of_gset A]≡ N⌝ ∧
-        t ⤇ run: (subst (of_val <$> σ) (td_expr U)) ∗ int_s_wait_pre iτs' iηs' U N' σ.
-  End HeapInterpretation.
-
-  Section Interpretations.
-    Context `{implStateG Σ, specStateG Σ, axiomaticIrisG Σ, taskDataG Σ} (c0: cfg).
-    Implicit Type N: name_map.
-    Implicit Type D: conn_map.
-    Implicit Type x: val.
-    Implicit Type d: val.
-    Local Open Scope I.
-    
-    Fixpoint int_s_type τ: @int_type Σ :=
-      match τ with
-      | tbool => int_s_bool
-      | tunit => int_s_unit
-      | tref ξ => int_s_ref ξ
-      | ttask ξ A τ => int_s_promise ξ
-      end.
-    Fixpoint int_s_heap_approx iη η: @int_heap Σ :=
-      match η with
-      | hemp => int_s_emp
-      | hstar η η' => int_s_star (int_s_heap_approx iη η) (int_s_heap_approx iη η')
-      | hpt ξ τ => int_s_pt ξ (int_s_type τ)
-      | hwait ξ A η => int_s_wait int_s_type iη ξ A η
-      end.
-    Fixpoint int_s_heap_rec n η :=
-      match n return @int_heap Σ with
-      | O => int_s_heap_approx (λ _ _ _, False%I) η
-      | S n => int_s_heap_approx (int_s_heap_rec n) η
-      end.
-    Definition heap_depth N n η :=
-      he_all_tasks (λ ξ, ∀ t γ, ⌜N !! t = Some (Task t γ)⌝ → depth N n γ) η.
-    Definition int_s_heap η: @int_heap Σ := λ D N, ∃ n, int_s_heap_rec n η D N.
-
-    Fixpoint int_i_type τ: @int_type Σ :=
-      match τ with
-      | tbool => int_i_bool
-      | tunit => int_i_unit
-      | tref ξ => int_i_ref ξ
-      | ttask ξ A τ => int_i_promise c0 int_s_type int_s_type int_s_heap int_s_heap
-                                     ξ A τ (int_i_type τ)
-      end.
-    Fixpoint int_i_heap η: @int_heap Σ :=
-      match η with
-      | hemp => int_i_emp
-      | hstar η η' => int_i_star (int_i_heap η) (int_i_heap η')
-      | hpt ξ τ => int_i_pt ξ (int_i_type τ)
-      | hwait ξ A η => int_i_wait ξ A η (int_i_heap η)
-      end.
-
-    Definition int_s_env := intΓ int_s_type.
-    Definition int_i_env := intΓ int_i_type.
-    
-    (** Basic properties of interpretation *)
-    Global Instance int_s_type_persistent τ d N v:  PersistentP (int_s_type τ d N v).
-    Proof. destruct τ; apply _. Qed.
-    Global Instance int_i_type_persistent τ d N v:  PersistentP (int_i_type τ d N v).
-    Proof. destruct τ; apply _. Qed.
-    Global Instance int_s_env_persistent Γ D N σ: PersistentP (int_s_env Γ D N σ).
-    Proof. apply _. Qed.
-    Global Instance int_i_env_persistent Γ D N σ: PersistentP (int_i_env Γ D N σ).
-    Proof. apply _. Qed.
-
-    Global Instance int_s_type_local τ:
-      Proper ((=) ==> overlap (names τ) ==> (=) ==> (⊣⊢)) (int_s_type τ).
-    Proof.
-      induction τ; intros d ? <- N N' eqN x ? <-; cbn; try done.
-      - rewrite /int_s_ref /int_i_ref.
-        rewrite eqN; first done.
-        cbn; set_solver.
-      - rewrite /int_s_promise.
-        rewrite eqN; first done.
-        cbn -[union]; set_solver.
-    Qed.
-    
-    Global Instance wait_proper t: Proper (pointwise_relation _ (≡) ==> (≡)) (@wait Σ t).
-    Proof.
-      intros ϕ ϕ' eqϕ.
-      rewrite equiv_dist; intro.
-      apply wait_nonexpansive; intro v.
-      rewrite eqϕ; done.
-    Qed.
-
-    Global Instance int_i_type_local τ:
-      Proper ((=) ==> overlap (names τ) ==> (=) ==> (⊣⊢)) (int_i_type τ).
-    Proof.
-      induction τ; intros d ? <- N N' eqN x ? <-; cbn; try done.
-      - rewrite /int_i_ref eqN; first done.
-        cbn; set_solver.
-      - rewrite /int_i_promise /int_i_promise_body /ip_impl.
-        rewrite (eqN ξ); last set_solver.
-        do 21 f_equiv.
-        apply (overlap_iff (of_gset (names (ttask ξ A τ)))).
-        + cbn -[union]; intro.
-          rewrite elem_of_difference !elem_of_of_gset.
-          set_solver.
-        + intro; rewrite elem_of_of_gset; auto.
-    Qed.
-
-    Definition names_heap (η: types.heap): gset conn_name := of_list (name <$> (elements (names η))).
-    Lemma elem_of_names_heap (d: conn_name) η:
-      (d ∈ names_heap η ↔ ∃ ξ: gname, d = name ξ ∧ ξ ∈ names η)%type.
-    Proof.
-      rewrite /names_heap elem_of_of_list elem_of_list_fmap.
-      f_equiv; intro ξ. by rewrite elem_of_elements.
-    Qed.
-
-    Lemma names_heap_star η η': (names_heap (η ⊗ η') ≡ names_heap η ∪ names_heap η')%C.
-    Proof.
-      rewrite /names_heap => ξ.
-      rewrite elem_of_union !elem_of_of_list !elem_of_list_fmap /=.
-      setoid_rewrite elem_of_elements.
-      change (names (hstar η η')) with (names η ∪ names η').
-      setoid_rewrite elem_of_union.
-      split.
-      - intros [? [? [?|?]]]; eauto.
-      - intros [[? [??]]|[? [??]]]; eauto.
-    Qed.
-    
-    Lemma int_s_heap_approx_local
-          iη (iη_proper: ∀ (η: types.heap),
-                 Proper (overlap (names_heap η) ==> overlap (names η) ==> (⊣⊢)) (iη η)) η:
-      Proper (overlap (names_heap η) ==> overlap (names η) ==> (⊣⊢)) (int_s_heap_approx iη η).
-    Proof.
-      induction η; intros D D' eqD N N' eqN; cbn.
-      - done.
-      - rewrite /int_s_star /int_i_star.
-        f_equiv; [apply IHη1|apply IHη2].
-        all: eapply overlap_mono; eauto.
-        all: cbn.
-        1,3: rewrite names_heap_star.
-        all: clear; set_solver.
-      - rewrite /int_s_pt.
-        setoid_rewrite (eqN ξ); last by set_solver.
-        rewrite eqD; cycle 1.
-        { rewrite /names_heap elem_of_of_list elem_of_list_fmap.
-          exists ξ; split; auto.
-          rewrite elem_of_elements; set_solver. }
-        enough (∀ d v, int_s_type τ d N v ⊣⊢ int_s_type τ d N' v) as eqint.
-        { by setoid_rewrite eqint. }
-        intros; apply int_s_type_local; auto.
-        eapply overlap_mono; eauto.
-        set_solver.
-      - rewrite /int_s_wait /=.
-        do 10 f_equiv.
-        rewrite (eqN ξ); last set_solver.
-        do 4 f_equiv.
-        apply (overlap_iff (of_gset (names (hwait ξ A η)))); eauto.
-        + intro ξ'.
-          rewrite elem_of_difference !elem_of_of_gset.
-          set_solver.
-        + intros ξ'; rewrite elem_of_of_gset; auto.
-    Qed.
-
-    Lemma int_s_heap_rec_local n: ∀ η,
+  Lemma int_s_heap_rec_local n: ∀ η,
       Proper (overlap (names_heap η) ==> overlap (names η) ==> (⊣⊢)) (int_s_heap_rec n η).
-    Proof.
-      induction n as [|n IH]; intros; cbn; apply int_s_heap_approx_local; auto.
-      solve_proper.
-    Qed.
+  Proof.
+    induction n as [|n IH]; intros; cbn; apply int_s_heap_approx_local; auto.
+    solve_proper.
+  Qed.
 
-    Lemma int_s_heap_local η:
-      Proper (overlap (names_heap η) ==> overlap (names η) ==> (⊣⊢)) (int_s_heap η).
-    Proof.
-      intros D D' eqD N N' eqN.
-      rewrite /int_s_heap.
-      f_equiv; intro n.
-      apply int_s_heap_rec_local; done.
-    Qed.
-    
-    Lemma int_i_heap_local η:
-      Proper (overlap (names_heap η) ==> overlap (names η) ==> (⊣⊢)) (int_i_heap η).
-    Proof.
-      induction η; intros D D' eqD N N' eqN; cbn.
-      - done.
-      - rewrite /int_s_star /int_i_star.
-        f_equiv; [apply IHη1|apply IHη2].
-        all: eapply overlap_mono; eauto.
-        all: cbn.
-        1,3: rewrite names_heap_star.
-        all: clear; set_solver.
-      - rewrite /int_i_pt.
-        rewrite (eqN ξ); last set_solver.
-        rewrite (eqD (name ξ)).
-        2: rewrite /names_heap elem_of_of_list elem_of_list_fmap.
-        2: eexists; split; eauto.
-        2: rewrite elem_of_elements; set_solver.
-        assert (N ≡[ names τ ]≡ N') as eqN'.
-        { intros ξ' inξ; apply eqN; set_solver. }
-        enough (∀ d v, int_i_type τ d N v ⊣⊢ int_i_type τ d N' v) as eqτ.
-        { by setoid_rewrite eqτ. }
-        intros; by apply int_i_type_local.
-      - rewrite /int_i_wait /int_i_wait_body.
-        rewrite (eqN ξ); last set_solver.
-        enough (∀ N'', N ≡[ of_gset (names η) ∖ of_gset A ]≡ N'' ↔
-                         N' ≡[ of_gset (names η) ∖ of_gset A ]≡ N'')
-          as eqN'.
-        { by setoid_rewrite eqN'. }
-        intros.
-        enough (N''≡[ of_gset (names η) ∖ of_gset A ]≡ N ↔
-                   N'' ≡[ of_gset (names η) ∖ of_gset A ]≡ N')
-          as ov.
-        { split; intros eqN' ξ' inξ'; symmetry; apply ov; eauto; done. }
-        apply (overlap_iff (of_gset (names (hwait ξ A η)))).
-        + intro; rewrite elem_of_difference !elem_of_of_gset; set_solver.
-        + intros ?; rewrite elem_of_of_gset; auto.
-    Qed.
+  Lemma int_s_heap_local η:
+    Proper (overlap (names_heap η) ==> overlap (names η) ==> (⊣⊢)) (int_s_heap η).
+  Proof.
+    intros D D' eqD N N' eqN.
+    rewrite /int_s_heap.
+    f_equiv; intro n.
+    apply int_s_heap_rec_local; done.
+  Qed.
+  
+  Lemma int_i_heap_local η:
+    Proper (overlap (names_heap η) ==> overlap (names η) ==> (⊣⊢)) (int_i_heap η).
+  Proof.
+    induction η; intros D D' eqD N N' eqN; cbn.
+    - done.
+    - rewrite /int_s_star /int_i_star.
+      f_equiv; [apply IHη1|apply IHη2].
+      all: eapply overlap_mono; eauto.
+      all: cbn.
+      1,3: rewrite names_heap_star.
+      all: clear; set_solver.
+    - rewrite /int_i_pt.
+      rewrite (eqN ξ); last set_solver.
+      rewrite (eqD (name ξ)).
+      2: rewrite /names_heap elem_of_of_list elem_of_list_fmap.
+      2: eexists; split; eauto.
+      2: rewrite elem_of_elements; set_solver.
+      assert (N ≡[ names τ ]≡ N') as eqN'.
+      { intros ξ' inξ; apply eqN; set_solver. }
+      enough (∀ d v, int_i_type τ d N v ⊣⊢ int_i_type τ d N' v) as eqτ.
+      { by setoid_rewrite eqτ. }
+      intros; by apply int_i_type_local.
+    - rewrite /int_i_wait /int_i_wait_body.
+      rewrite (eqN ξ); last set_solver.
+      enough (∀ N'', delete ξ N ≡[ names η ∖ A ]≡ N'' ↔
+                       delete ξ N' ≡[ names η ∖ A ]≡ N'')
+        as eqN'.
+      { by setoid_rewrite eqN'. }
+      intro.
+      rewrite -!(symmetry_iff (overlap (names η ∖ A)) N'').
+      apply (overlap_iff (names (hwait ξ A η))).
+      + apply union_subseteq_r.
+      + intros ξ' inξ'.
+        destruct (decide (ξ = ξ')) as [<-|neq].
+        * by rewrite !lookup_delete.
+        * rewrite !lookup_delete_ne; auto.
+  Qed.
 
-    Definition env_names (Γ: env): gset conn_name := of_list (var <$> fst <$> map_to_list Γ).
-    Lemma intΓ_local (ϕ: type → @int_type Σ)
-          (ϕ_local: ∀ τ, Proper ((=) ==> overlap (names τ) ==> (=) ==> (⊣⊢)) (ϕ τ)) Γ:
-      Proper (overlap (env_names Γ) ==> overlap (names Γ) ==> (=) ==> (⊣⊢)) (intΓ ϕ Γ).
-    Proof.
-      intros D D' eqD N N' eqN σ ? <-.
-      rewrite /intΓ.
-      f_equiv.
-      assert (∀ (x: string), is_Some (Γ !! x) → (is_Some (D!!var x) ↔ is_Some (D'!!var x)))
-        as eqD'.
-      { intros x [τ mtx].
-        rewrite eqD; first done.
-        rewrite /env_names elem_of_of_list -list_fmap_compose elem_of_list_fmap.
-        exists (x,τ); split; auto.
-        rewrite elem_of_map_to_list; done. }
-      f_equiv.
-      { f_equiv.
-        apply forall_proper; intro.
-        specialize (eqD' x); tauto. }
-      f_equiv; intro x.
-      f_equiv; intro τ.
-      f_equiv; intro v.
-      f_equiv; intro d.
-      destruct (Γ!!x) as [τ'|] eqn:mtx.
-      2: iSplit; iIntros "pre"; iIntros ([[=]?]).
-      rewrite (eqD (var x)); cycle 1.
-      { rewrite /env_names elem_of_of_list -list_fmap_compose elem_of_list_fmap.
-        exists (x,τ'); split; auto; rewrite elem_of_map_to_list; done. }
-      assert ({τ' = τ} + {τ' ≠ τ}) as [->|neq].
-      { decide equality.
-        1, 3: apply (decide (ξ = ξ0)).
-        apply (decide (A = A0)). }
-      2: iSplit; iIntros "pre"; iIntros ([??]); congruence.
-      f_equiv.
-      apply ϕ_local; auto.
-      eapply (overlap_mono (names Γ)); eauto.
-      intros ξ inξ.
-      rewrite /names /Names_instance_2.
-      clear eqD eqN eqD'.
-      induction Γ using map_ind.
-      { rewrite lookup_empty in mtx; done. }
-      destruct (decide (i=x)) as [->|neq].
-      + rewrite big_opM_insert; last done.
-        rewrite lookup_insert in mtx.
-        injection mtx as ->.
-        set_solver.
-      + rewrite big_opM_insert; last done.
-        rewrite lookup_insert_ne in mtx; last done.
-        set_solver.
-    Qed.
-  End Interpretations.
-End TypeTranslation.
+  Lemma intΓ_local (ϕ: type → @int_type Σ)
+        (ϕ_local: ∀ τ, Proper ((=) ==> overlap (names τ) ==> (=) ==> (⊣⊢)) (ϕ τ)) Γ:
+    Proper (overlap (names_env Γ) ==> overlap (names Γ) ==> (=) ==> (⊣⊢)) (intΓ ϕ Γ).
+  Proof.
+    intros D D' eqD N N' eqN σ ? <-.
+    rewrite /intΓ.
+    assert (pure_l_and: ∀ P P' (Q Q': iProp Σ) (eqP: (P ↔ P')%type) (eqQ: P → Q ⊣⊢ Q'),
+               ⌜P⌝ ∧ Q ⊣⊢ ⌜P'⌝ ∧ Q').
+    { intros; rewrite -eqP.
+      iSplit; iIntros "[% pre]"; rewrite eqQ; auto. }
+    apply pure_l_and.
+    { apply and_iff_compat_l, forall_proper; intro.
+      destruct (decide (is_Some (Γ!!x))) as [[τ tyx]|]; last tauto.
+      rewrite (eqD (var x)); first done.
+      rewrite elem_of_names_env.
+      exists x; eauto. }
+    intros [domσ domD].
+    f_equiv; intro x.
+    f_equiv; intro τ.
+    f_equiv; intro v.
+    f_equiv; intro d.
+    destruct (decide (Γ!!x = Some τ)) as [mt|].
+    2: iSplit; iIntros "_ %"; intuition discriminate.
+    assert (var x ∈ names_env Γ) as in_var_x.
+    { rewrite elem_of_names_env; exists x; rewrite mt; eauto. }
+    rewrite (eqD (var x)); last done.
+    f_equiv.
+    apply ϕ_local; try done.
+    eapply overlap_mono.
+    2,3,4: done.
+    intro ξ.
+    rewrite env_elem_of_names.
+    exists x,τ; auto.
+  Qed.
+
+  Lemma int_i_env_local Γ: 
+    Proper (overlap (names_env Γ) ==> overlap (names Γ) ==> (=) ==> (⊣⊢)) (int_i_env  Γ).
+  Proof. apply intΓ_local, int_i_type_local. Qed.
+  Lemma int_s_env_local Γ: 
+    Proper (overlap (names_env Γ) ==> overlap (names Γ) ==> (=) ==> (⊣⊢)) (int_s_env  Γ).
+  Proof. apply intΓ_local, int_s_type_local. Qed.
+  
+  Lemma int_s_heap_approx_mono ϕ ϕ' (mono: ∀ η D N, ϕ η D N -∗ ϕ' η D N) η:
+    ∀ D N, int_s_heap_approx ϕ η D N -∗ int_s_heap_approx ϕ' η D N.
+  Proof.
+    induction η; cbn.
+    - iIntros (??) "$".
+    - iIntros (D N) "[I1 I2]".
+      iSplitL "I1".
+      + iApply (IHη1 with "I1").
+      + iApply (IHη2 with "I2").
+    - iIntros (??) "$".
+    - iIntros (D N).
+      rewrite /int_s_wait /int_s_wait_pre.
+      iIntros "pre".
+      iDestruct "pre" as (t γ U N' σ) "[pre [move [env wait]]]".
+      iExists t,γ,U,N',σ; iFrame.
+      iApply (mono with "wait").
+  Qed.
+  Lemma int_s_heap_rec_S n: ∀ η D N, int_s_heap_rec n η D N -∗ int_s_heap_rec (S n) η D N.
+  Proof.
+    rewrite -Nat.add_1_r.
+    induction n as [|n IH]; cbn.
+    all: iIntros (η D N) "pre"; iApply (int_s_heap_approx_mono with "pre").
+    - iIntros (???) "[]".
+    - exact IH.
+  Qed.
+  
+  Lemma int_s_heap_rec_mono n n' (len: n ≤ n'):
+    ∀ η D N, int_s_heap_rec n η D N -∗ int_s_heap_rec n' η D N.
+  Proof.
+    induction len.
+    { iIntros (???) "$". }
+    iIntros (η D N) "pre".
+    iApply (int_s_heap_rec_S with "[-]").
+    iApply (IHlen with "pre").
+  Qed.
+End Interpretations.
