theories/delayed.v
@@ -1,0 +1,1365 @@
+From iris.proofmode Require Import tactics.
+From iris.base_logic.lib Require Import invariants.
+From iris.algebra Require Import agree auth excl updates local_updates.
+From esop Require Import typetranslation corecalculus specification types overlap oneshot.
+From stdpp Require Import gmap set coPset.
+
+Module Delayed(AxSem: AxiomaticSemantics).
+  Module Import Axiomatics := AxSem <+ AxiomaticFacts.
+  Instance: WaitPermissions :=
+    Build_WaitPermissions axiomaticIrisG _ (@wait).
+
+  Section Definitions.
+    Context `{specStateG Σ} {Hiris: wp_axiomaticIrisG Σ} `{taskDataG Σ, InitialConfiguration}.
+    Instance: axiomaticIrisG Σ := Hiris.
+    Typeclasses Transparent axiomaticIrisG.
+    Local Open Scope I.
+
+    Definition simulation := simulation_body int_s_type int_s_heap.
+    
+    Definition delayed_typed Γ η e e' A τ η' :=
+      ∀ D N σ,
+        (int_i_env Γ D N σ ∗ int_i_heap η D N)
+          -∗ WP subst (of_val <$> σ) e
+          {{ xᵢ, ∃ Nᵢ' D' d', ⌜N ≡[ not_new A ]≡ Nᵢ' ∧ D' !! RET = Some d'⌝ ∗
+                             int_i_type τ d' Nᵢ' xᵢ ∗
+                             int_i_heap η' D' Nᵢ' ∗
+                             □simulation Γ e' η A τ η' D D' }}.
+    Record delayed_simulation U Γ (η: heap) e e' A (τ: type) (η': heap) :=
+      Delayed {
+          ds_used_names: names Γ ∪ names η ⊆ U;
+          ds_type_e: typing U Γ e η A τ η';
+          ds_type_e': typing U Γ e' η A τ η';
+          ds_sim: delayed_typed Γ η e e' A τ η'
+        }.
+
+    (** Meta-theory: The binding lemma *)
+    Definition strengthen Γ x (d: val) (D D': conn_map) := <[var x:=d]>(D ~[names_env Γ]~> D').
+    
+    Lemma strengthen_env_generic
+          (int_ty: type → @int_type Σ) ϕ
+          (Γ: env) (τ: type) x D D' v d (σ: gmap string val) N N'
+          (L: gset conn_name) (disj: names_env Γ ⊥ L) (notin: var x ∉ L) O (Osub: names Γ ⊆ O)
+          (ϕ_local: Proper (overlap L ==> (⊣⊢)) (ϕ N'))
+          (int_local: ∀ τ, Proper (eq ==> overlap (names τ) ==> eq ==> (⊣⊢)) (int_ty τ)):
+      intΓ int_ty Γ D N σ -∗ (⌜N ≡[O]≡ N'⌝ ∗ int_ty τ d N' v ∗ ϕ N' D') -∗
+           let D'' := strengthen Γ x d D D' in
+           intΓ int_ty (<[x:=τ]>Γ) D'' N' (<[x:=v]>σ) ∗ ϕ N' D''.
+    Proof.
+      iIntros "intΓ [eqN [intτ ϕ]]".
+      iDestruct "eqN" as %eqN; cbn.
+      iSplitR "ϕ".
+      { iDestruct "intΓ" as "[dom intΓ]".
+        iDestruct "dom" as %[domσ domD].
+        iSplit.
+        { iPureIntro; split.
+          { intros y.
+            destruct (decide (x=y)) as [<-|neq].
+            - rewrite !lookup_insert; split; eauto.
+            - rewrite !lookup_insert_ne; eauto. }
+          { intros y.
+            destruct (decide (x=y)) as [<-|neq].
+            { rewrite !lookup_insert; eauto. }
+            rewrite !lookup_insert_ne. 2,3: congruence.
+            intros indom.
+            rewrite lookup_merge_along_in; first eauto.
+            rewrite elem_of_names_env.
+            exists y; eauto. }
+        }
+        iIntros (x' τ' v' d' [lookupτ [lookupv lookupd]]).
+        destruct (decide (x=x')) as [<-|neq].
+        { rewrite lookup_insert in lookupd; injection lookupd as <-.
+          rewrite lookup_insert in lookupv; injection lookupv as <-.
+          rewrite lookup_insert in lookupτ; injection lookupτ as <-.
+          iFrame.
+        } {
+          rewrite lookup_insert_ne in lookupτ; last done.
+          rewrite lookup_insert_ne in lookupd; last congruence.
+          rewrite lookup_insert_ne in lookupv; last done.
+          rewrite (int_local τ' d' d' eq_refl N' N); last done.
+          - iApply ("intΓ" $! x' τ' v' d').
+            iPureIntro; intuition.
+            rewrite lookup_merge_along_in in lookupd; auto.
+            rewrite elem_of_names_env; eauto.
+          - symmetry.
+            eapply overlap_mono.
+            2,3,4: done.
+            trans (names Γ); auto.
+            intros ξ.
+            rewrite env_elem_of_names.
+            exists x', τ'; eauto. }
+      }
+      enough (overlap L D' (<[var x:=d]>(D ~[names_env Γ]~> D'))) as ov.
+      { by rewrite /strengthen -ov. }
+      intros n inn.
+      rewrite lookup_insert_ne.
+      2: by intros <-.
+      rewrite lookup_merge_along_not_in; first done.
+      set_solver.
+    Qed.
+
+    Lemma good_overlap A A': not_new (A ∪ A') ⊆ not_new A ∩ not_new A'.
+    Proof.
+      intro ξ.
+      rewrite /not_new elem_of_intersection !elem_of_difference !elem_of_of_gset
+              not_elem_of_union.
+      tauto.
+    Qed.
+
+    Lemma overlap_trans {X} A A' (N N' N'': gmap gname X):
+      N ≡[not_new A]≡ N' → N' ≡[not_new A']≡ N'' →
+      N ≡[not_new (A ∪ A')]≡ N''.
+    Proof.
+      intros ov1 ov2.
+      pose proof (good_overlap A A').
+      etrans.
+      all: eapply overlap_mono.
+      2,3,6,7: done.
+      2,4: eassumption.
+      all: set_solver.
+    Qed.
+
+    Local Open Scope I.
+    Context `{∀ t, Proper (pointwise_relation _ (⊣⊢) ==> (⊣⊢)) (wait t)}.
+    
+    Lemma existential_part (x: string) e K Γ τ₁ τ₂ η₁ η₂ η₃ A₁ A₂ (D₁ D₂ D₃: conn_map) d
+          (d_good: D₂!!RET = Some d) (Γ_names_good: names Γ ⊥ A₁)
+          (x_fresh: ∀ e', subst_ctx (<[x:=e']>∅) K = K):
+      simulation Γ e η₁ A₁ τ₁ η₂ D₁ D₂
+                 -∗ simulation (<[x:=τ₁]>Γ) (fill_ctx x K) η₂ A₂ τ₂ η₃ (strengthen Γ x d D₁ D₂) D₃
+                 -∗ simulation Γ (fill_ctx e K) η₁ (A₁ ∪ A₂) τ₂ η₃ D₁ D₃.
+    Proof.
+      iIntros "sime simK".
+      iIntros (N σ p K') "#ctx [#Γ pre] step".
+      rewrite subst_fill fill_ctx_app.
+      iMod ("sime" $! N σ p (subst_ctx (of_val <$> σ) K++K')
+              with "ctx [$Γ $pre] step") as (v₁) "[post step]".
+      iDestruct "post" as (d' N') "[props [ty pre]]".
+      iDestruct "props" as %[eqN eqd].
+      replace d' with d in * by congruence.
+      iPoseProof (strengthen_env_generic int_s_type (λ N D, int_s_heap η₂ D N) Γ τ₁ x D₁ D₂
+                                         v₁ d σ N N' (names_heap η₂))
+        as "str".
+      { intro n.
+        rewrite elem_of_names_env.
+        rewrite /names_heap elem_of_of_list elem_of_list_fmap.
+        intros [? [-> _]] [? [[=] _]]. }
+      { rewrite /names_heap elem_of_of_list elem_of_list_fmap.
+        intros [? [[=] _]]. }
+      { done. }
+      { intros D D' eqD. by apply int_s_heap_local. }
+      { apply int_s_type_local. }
+      iDestruct ("str" with "Γ [$ty $pre]") as "[Γ' pre]".
+      { iPureIntro.
+        apply overlap_cast.
+        eapply overlap_mono.
+        2-4: done.
+        intro ξ.
+        rewrite elem_of_of_gset /not_new elem_of_difference elem_of_of_gset.
+        set_solver. }
+      rewrite -fill_ctx_app -(subst_val v₁ (of_val <$> σ)) -subst_fill.
+      iMod ("simK" $! N' (<[x := v₁]>σ) p K' with "ctx [$Γ' $pre] [step]")
+        as (v₂) "[post step]".
+      { rewrite fmap_insert subst_insert_r; auto using val_closed.
+        rewrite (subst_fill (<[x:=of_val v₁]>∅)) x_fresh /= lookup_insert //. }
+      iDestruct "post" as (d'' N'') "[eqs post]".
+      iModIntro.
+      iExists v₂; iFrame.
+      iExists d'', N''; iFrame.
+      iDestruct "eqs" as %[eqN' eqd'].
+      iPureIntro; split; auto.
+      eapply overlap_trans; eauto.
+    Qed.
+
+    Lemma wp_bind_inv K E e ϕ:
+      WP fill_ctx e K @ E {{ ϕ }} ⊢ WP e @ E {{ v, WP fill_ctx (of_val v) K @ E {{ ϕ }} }}.
+    Proof.
+      revert e ϕ.
+      induction K using rev_ind; iIntros (e ϕ) "wp"; cbn.
+      { iApply (wp_wand with "wp").
+        iIntros (v); iApply wp_value'. }
+      rewrite -!fill_ctx_app /=.
+      iPoseProof (wp_bind_item_inv with "wp") as "wp".
+      iPoseProof (IHK with "wp") as "wp".
+      iApply (wp_wand with "wp").
+      iIntros (v) "wp".
+      rewrite -fill_ctx_app /=.
+      iApply wp_bind_item; done.
+    Qed.
+    
+    Lemma wp_bind K E e ϕ:
+      WP e@E {{ v, WP fill_ctx (of_val v) K @ E {{ ϕ }} }}
+         -∗ WP fill_ctx e K @ E {{ ϕ }}.
+    Proof.
+      revert e ϕ.
+      induction K using rev_ind; iIntros (e ϕ) "wp"; cbn.
+      { iApply (wp_strong_mono with "[$wp]"); first done.
+        iIntros (v); iApply wp_value_inv. }
+      rewrite -!fill_ctx_app /=.
+      iApply wp_bind_item.
+      iApply IHK.
+      iApply (wp_wand with "wp").
+      iIntros (v) "wp".
+      iApply wp_bind_item_inv.
+      rewrite -fill_ctx_app; done.
+    Qed.
+    
+    Lemma universal_part (x: string) e e' K K' Γ τ₁ τ₂ η₁ η₂ η₃ A₁ A₂
+          (Γ_names_good: names Γ ⊥ A₁)
+          (x_fresh: ∀ e', subst_ctx (<[x:=e']>∅) K = K)
+          (x_fresh': ∀ e', subst_ctx (<[x:=e']>∅) K' = K'):
+      delayed_typed Γ η₁ e e' A₁ τ₁ η₂
+                    -∗ delayed_typed (<[x:=τ₁]>Γ) η₂ (fill_ctx x K) (fill_ctx x K') A₂ τ₂ η₃
+                    -∗ delayed_typed Γ η₁ (fill_ctx e K) (fill_ctx e' K') (A₁ ∪ A₂) τ₂ η₃.
+    Proof.
+      iIntros "dele delK".
+      iIntros (D Ni σi) "[#intΓ intη]".
+      rewrite subst_fill.
+      iApply wp_bind.
+      iSpecialize ("dele" $! D Ni σi with "[$intΓ $intη]").
+      iApply (wp_wand with "dele [-]").
+      iIntros (v) "post".
+      iDestruct "post" as (Ni' D' d') "[rel [intτ [intη' #sim]]]".
+      replace (fill_ctx (of_val v) (subst_ctx (of_val <$> σi) K))
+        with (subst (of_val <$> (<[x:=v]>σi)) (fill_ctx x K)); cycle 1.
+      { rewrite fmap_insert subst_insert_r; auto using val_closed.
+        rewrite subst_fill /= lookup_insert x_fresh -(subst_val _ (of_val <$> σi)) -subst_fill.
+        rewrite subst_val //. }
+      iDestruct "rel" as %[eqN eqd].
+      iSpecialize ("delK" $! (strengthen Γ x d' D D') Ni' (<[x:=v]>σi) with "[intτ intη']").
+      { iApply (strengthen_env_generic
+                  int_i_type (λ N D, int_i_heap η₂ D N)
+                  Γ τ₁ x D D' v d' σi Ni Ni' (names_heap η₂)
+                  with "intΓ [intτ intη']").
+        - intro n.
+          rewrite /names_env /names_heap !elem_of_of_list !elem_of_list_fmap.
+          intros [? [-> _]] [? [[=] _]].
+        - rewrite /names_heap elem_of_of_list elem_of_list_fmap.
+          intros [? [[=] _]].
+        - done.
+        - intros D₁ D₂ eqD.
+          apply int_i_heap_local; auto.
+          done.
+        - iFrame.
+          iPureIntro.
+          apply overlap_cast.
+          eapply overlap_mono.
+          2-4: done.
+          intro ξ.
+          rewrite /not_new elem_of_difference !elem_of_of_gset.
+          set_solver.
+      }
+      iApply (wp_wand with "delK").
+      iIntros (v') "post".
+      iDestruct "post" as (Ni'' D'' d'') "[pure [intτ [intη #sim']]]".
+      iDestruct "pure" as %[eqN' eqD'].
+      iExists Ni'', D'', d''; iFrame.
+      iSplit.
+      { iPureIntro; split; auto.
+        eapply overlap_trans; eauto. }
+      iAlways.
+      iApply (existential_part with "sim sim'"); auto.
+    Qed.
+
+    Lemma delayed_bind
+          (x: string) e e' K K' Γ τ₁ τ₂ η₁ η₂ η₃ U A₁ A₂
+          (x_fresh: ∀ e', subst_ctx (<[x:=e']>∅) K = K)
+          (x_fresh': ∀ e', subst_ctx (<[x:=e']>∅) K' = K')
+          (dele: delayed_simulation U Γ η₁ e e' A₁ τ₁ η₂)
+          (delK: delayed_simulation (U ∪ A₁) (<[x:=τ₁]>Γ) η₂ (fill_ctx x K) (fill_ctx x K') A₂ τ₂ η₃):
+      delayed_typed Γ η₁ (fill_ctx e K) (fill_ctx e' K') (A₁ ∪ A₂) τ₂ η₃.
+    Proof.
+      destruct dele as [namese tye tye' dele].
+      destruct delK as [namesK tyK tyK' delK].
+      iApply universal_part.
+      2,3: done.
+      2: iApply dele.
+      2: iApply delK.
+      apply typing_good_names in tye.
+      - destruct tye as [disj _].
+        clear -disj namese.
+        set_solver.
+      - intros x' τ' mt ξ inξ.
+        apply namese, elem_of_union, or_introl, env_elem_of_names.
+        eauto.
+      - clear -namese; set_solver.
+    Qed.
+
+    (** Meta theory: The framing lemma *)
+    Definition frame ηf (D D': conn_map): conn_map := D ~[names_heap ηf]~> D'.
+
+    Lemma frame_generic          
+          (int_ty: type → @int_type Σ) (int_he: heap → @int_heap Σ) τ (η ηf: heap)          
+          D D' d v (N N': name_map) (nov: N ≡[names ηf]≡ N')
+          (int_he_split: ∀ D'' N'',
+              int_he (hstar η ηf) D'' N'' ⊣⊢ int_he η D'' N'' ∗ int_he ηf D'' N'')
+          (int_he_local: ∀ η,
+              Proper (overlap (names_heap η) ==> overlap (names η) ==> (≡)) (int_he η))
+          (disj: names η ⊥ names ηf):
+      int_he ηf D N -∗ (⌜D' !! RET = Some d⌝ ∗ int_ty τ d N' v ∗ int_he η D' N') -∗
+             (⌜frame ηf D D' !! RET = Some d⌝) ∗
+             int_ty τ d N' v ∗ int_he (hstar η ηf) (frame ηf D D') N'.
+    Proof.
+      iIntros "frame [eqd [type heap]]".
+      iFrame.
+      iSplitL "eqd".
+      { iDestruct "eqd" as %eqd.
+        iPureIntro.
+        rewrite /frame lookup_merge_along_not_in //.
+        rewrite /names_heap elem_of_of_list elem_of_list_fmap.
+        intros [? [[=] _]]. }
+      rewrite int_he_split.
+      iSplitL "heap".
+      - iApply (int_he_local with "heap"); last done.
+        apply overlap_merge_along_r.
+        rewrite /names_heap => [n].
+        rewrite !elem_of_of_list !elem_of_list_fmap.
+        intros [ξ [-> inηf%elem_of_elements]] [? [[=<-] inη%elem_of_elements]].
+        apply (disj ξ); done.
+      - iApply (int_he_local with "frame"); first apply overlap_merge_along_l.
+        done.
+    Qed.
+
+    Lemma int_s_rec_split n η η' D N:
+      int_s_heap_rec n (hstar η η') D N ⊣⊢ int_s_heap_rec n η D N ∗ int_s_heap_rec n η' D N.
+    Proof. destruct n; done. Qed.
+    
+    Lemma int_s_heap_split η η' D N:
+      int_s_heap (hstar η η') D N ⊣⊢ (int_s_heap η D N ∗ int_s_heap η' D N).
+    Proof.
+      iSplit.
+      { iIntros "pre".
+        iDestruct "pre" as (n) "pre".
+        rewrite int_s_rec_split.
+        iDestruct "pre" as "[pre pre']".
+        iSplitL "pre"; iExists n; iFrame.
+      } {
+        iIntros "[pre pre']".
+        iDestruct "pre" as (n) "pre".
+        iDestruct "pre'" as (n') "pre'".
+        iExists (max n n').
+        rewrite int_s_rec_split.
+        iSplitL "pre".
+        all: iApply int_s_heap_rec_mono; last iFrame.
+        all: auto with arith.
+      }
+    Qed.
+    
+    Lemma frame_existential Γ e (η: heap) A τ (η': heap) D D' D'' (ηf: heap)
+          (disj': names η' ⊥ names ηf) (disj: names η ⊥ names ηf) (disj'': names ηf ⊥ A):
+      simulation Γ e η A τ η' D D' -∗
+                 simulation Γ e (hstar η ηf) A τ (hstar η' ηf) (frame ηf D'' D) (frame ηf D'' D').
+    Proof.
+      iIntros "sim".
+      iIntros (N σ p K) "ctx [env pre] move".
+      rewrite int_s_heap_split.
+      iDestruct "pre" as "[pre frame]".
+      iMod ("sim" with "ctx [env pre] move") as (v) "[post move]".
+      { iSplitL "env".
+        - iApply (int_s_env_local with "env"). 2,3: done.
+          symmetry.
+          apply overlap_merge_along_r.
+          rewrite /names_heap /names_env => [n].
+          rewrite !elem_of_of_list !elem_of_list_fmap.
+          intros [? [-> _]] [? [[=] _]].
+        - iApply (int_s_heap_local with "pre"); last done.
+          symmetry.
+          apply overlap_merge_along_r.
+          rewrite /names_heap => [n].
+          rewrite !elem_of_of_list !elem_of_list_fmap.
+          intros [x [-> inη%elem_of_elements]] [? [[=<-] inηf%elem_of_elements]].
+          apply (disj x); auto. }
+      iDestruct "post" as (d N') "[eqs [type post]]".
+      iModIntro; iExists v; iFrame.
+      iDestruct "eqs" as %[eqN eqd].
+      iExists d, N'.
+      iPoseProof (frame_generic int_s_type int_s_heap τ η' ηf D'' D' d v N N'
+                    with "[frame] [$type $post]") as "post".
+      4,6: auto.
+      - apply overlap_cast.
+        eapply overlap_mono.
+        2-4: done.
+        intros ξ.
+        rewrite /not_new elem_of_difference !elem_of_of_gset.
+        set_solver.
+      - apply int_s_heap_split.
+      - intro; apply int_s_heap_local.
+      - iApply (int_s_heap_local with "frame"); last done.
+        symmetry; apply overlap_merge_along_l.
+      - iDestruct "post" as "[% [$$]]"; auto.
+    Qed.
+
+    Lemma simulation_local Γ e η A τ η':
+      Proper (overlap (names_env Γ ∪ names_heap η) ==> overlap ({[RET]} ∪ names_heap η') ==> (⊣⊢))
+             (simulation Γ e η A τ η').
+    Proof.
+      iIntros (D D' eqD E E' eqE).
+      rewrite /simulation /simulation_body /existential_triple.
+      f_equiv; intro N.
+      f_equiv; intro σ.
+      f_equiv; intro p.
+      f_equiv; intro K.
+      do 2 f_equiv.
+      { f_equiv.
+        - apply int_s_env_local.
+          2,3: done.
+          eapply overlap_mono.
+          2-4: done.
+          clear; set_solver.
+        - apply int_s_heap_local.
+          2,3: done.
+          eapply overlap_mono.
+          2-4: done.
+          clear; set_solver. }
+      do 3 f_equiv; intro v.
+      do 2 f_equiv; intro d.
+      f_equiv; intro N'.
+      f_equiv.
+      { rewrite (eqE RET); first done.
+        clear; set_solver. }
+      f_equiv.
+      apply int_s_heap_local; last done.
+      eapply overlap_mono.
+      2-4: done.
+      clear; set_solver.
+    Qed.
+    
+    Lemma closed_frame Γ e e' (η: heap) A τ (η' ηf: heap)
+          (disj': names η' ⊥ names ηf) (disj: names η ⊥ names ηf) (disj'': names ηf ⊥ A):
+      delayed_typed Γ η e e' A τ η' -∗
+                    delayed_typed Γ (hstar η ηf) e e' A τ (hstar η' ηf).
+    Proof.
+      iIntros "del".
+      iIntros (D N σ); cbn -[difference].
+      iIntros "[env [pre frame]]".
+      iSpecialize ("del" $! D N σ with "[$env $pre]").
+      iApply (wp_wand with "del").
+      iIntros (v) "post".
+      iDestruct "post" as (N' D' d') "[eqs [type [post sim]]]".
+      iExists N', (frame ηf D D'), d'.
+      iFrame.
+      iDestruct "eqs" as %[eqN eqD'].
+      iSplit.
+      { iPureIntro; split; auto.
+        rewrite /frame lookup_merge_along_not_in; first done.
+        rewrite /names_heap elem_of_of_list elem_of_list_fmap.
+        intros [? [[=] _]]. }
+      iSplitR "sim".
+      { iSplitL "post".
+        - iApply (int_i_heap_local with "post"); last done.
+          apply overlap_merge_along_r.
+          intro n.
+          rewrite /names_heap !elem_of_of_list !elem_of_list_fmap.
+          intros [ξ [-> inηf%elem_of_elements]] [? [[=<-] inη'%elem_of_elements]].
+          apply (disj' ξ); done.
+        - iApply (int_i_heap_local with "frame").
+          + apply overlap_merge_along_l.
+          + symmetry; apply overlap_cast.
+            eapply overlap_mono.
+            2-4: done.
+            intro ξ.
+            rewrite /not_new elem_of_difference !elem_of_of_gset.
+            clear -disj''; set_solver. }
+      iAssert (□simulation Γ e' (η ⊗ ηf) A τ (η' ⊗ ηf) (frame ηf D D) (frame ηf D D'))
+        with "[sim]" as "sim".
+      { iDestruct "sim" as "#sim"; iAlways; iApply (frame_existential with "sim"); auto. }
+      iDestruct "sim" as "#sim"; iAlways.
+      iApply (simulation_local with "sim"); last done.
+      intros n _.
+      rewrite /frame merge_along_cases.
+      destruct bool_decide; done.
+    Qed.
+    
+    (** Meta-theory: Strengthening the environment. *)
+    Definition restrict_subst' {A} (e: option A) (τ: option type) :=
+      match τ with Some _ => e | None => None end.
+    Definition restrict_subst {A} (Γ: env) (σ: gmap string A) := merge restrict_subst' σ Γ.
+    Instance: ∀ A, DiagNone (@restrict_subst' A).
+    Proof. done. Qed.
+    Lemma lookup_restrict_subst_is_Some {A} (Γ: env) (σ: gmap string A) x:
+      is_Some (restrict_subst Γ σ !! x) ↔ is_Some (Γ!!x) ∧ is_Some (σ!!x).
+    Proof.
+      rewrite /restrict_subst lookup_merge.
+      enough (∀ o, is_Some (restrict_subst' (σ!!x) o) ↔ is_Some o ∧ is_Some (σ !! x))
+        as -> by done.
+      intros [τ|]; cbn.
+      - intuition eauto.
+      - rewrite -!not_eq_None_Some; tauto.
+    Qed.
+    
+    Lemma restrict_env (int_ty: type → @int_type Σ) Γ Γ' D N σ (sub: Γ ⊆ Γ'):
+      intΓ int_ty Γ' D N σ -∗ intΓ int_ty Γ D N (restrict_subst Γ σ).
+    Proof.
+      rewrite /intΓ.
+      iIntros "[maps env]".
+      iDestruct "maps" as %[domσ domD].
+      iSplit.
+      { iPureIntro; split; intro.
+        - rewrite lookup_restrict_subst_is_Some.
+          split; last tauto.
+          intro inx; split; auto.
+          eapply domσ, lookup_weaken_is_Some; done.
+        - intro inx.
+          eapply domD, lookup_weaken_is_Some; done. }
+      iIntros (x τ v d) "pre".
+      iDestruct "pre" as %[eqτ [eqv eqd]].
+      iApply ("env" $! x τ v d).
+      iPureIntro.
+      repeat split; auto.
+      - by eapply lookup_weaken.
+      - by rewrite /restrict_subst lookup_merge eqτ in eqv.
+    Qed.
+
+    Lemma subst_restrict_with_type `(ty: typing U Γ e η A τ η'):
+      ∀ σ, subst (restrict_subst Γ σ) e = subst σ e.
+    Proof.
+      induction ty; intros; cbn.
+      1,2,3,6,7,8,9: congruence.
+      - by rewrite /restrict_subst lookup_merge Γx.
+      - rewrite IHty1; do 2 f_equal.
+        rewrite -(IHty2 (delete' x σ)); f_equal.
+        apply map_eq; intro y.
+        rewrite lookup_delete'_cases /restrict_subst !lookup_merge lookup_delete'_cases.
+        destruct (bool_decide_reflect (BNamed y ≠ x)) as [neqx|<-%dec_stable].
+        + rewrite /restrict_subst' /insert'.
+          destruct x; first done.
+          rewrite lookup_insert_ne; congruence.
+        + by destruct (insert' (BNamed y) τ₁ Γ !! y).
+    Qed.
+
+    Lemma restrict_env_fmap `(f: A → B) Γ m:
+      f <$> restrict_subst Γ m = restrict_subst Γ (f <$> m).
+    Proof.
+      apply map_eq; intro y.
+      rewrite /restrict_subst lookup_fmap !lookup_merge lookup_fmap /restrict_subst'.
+      match goal with |- f <$> match ?a with _ => _ end = _ => by destruct a end.
+    Qed.
+    
+    Lemma closed_strengthen U Γ Γ' e e' η A A' τ η'
+          (ty: typing U Γ e η A τ η')
+          (ty': typing U Γ e' η A τ η')
+          (subΓ: Γ ⊆ Γ') (subA: A ⊆ A'):
+      delayed_typed Γ η e e' A τ η' -∗ delayed_typed Γ' η e e' A' τ η'.
+    Proof.
+      iIntros "spec".
+      iIntros (D N σ) "[env pre]".
+      iSpecialize ("spec" $! D N (restrict_subst Γ σ) with "[env $pre]").
+      { by iApply (restrict_env with "env"). }
+      rewrite restrict_env_fmap (subst_restrict_with_type ty).
+      iApply (wp_wand with "spec").
+      iIntros (v) "post".
+      iDestruct "post" as (N' D' d') "[eqs [type [post sim]]]".
+      iExists N', D', d'; iFrame.
+      iDestruct "eqs" as %[eqN eqd].
+      iSplit.
+      { iPureIntro; split; auto.
+        eapply overlap_mono.
+        2-4: done.
+        clear -subA; red.
+        intro ξ.
+        rewrite /not_new !elem_of_difference !elem_of_of_gset.
+        set_solver. }
+      clear eqN N N' σ v.
+      iDestruct "sim" as "#sim"; iAlways.
+      iIntros (N σ p K) "ctx [env pre] move".
+      rewrite -(subst_restrict_with_type ty') -restrict_env_fmap.
+      iMod ("sim" $! N (restrict_subst Γ σ) p K with "ctx [env $pre] move") as (v) "[post move]".
+      { by iApply (restrict_env with "env"). }
+      iModIntro; iExists v; iFrame.
+      iDestruct "post" as (d N') "[eqs [type post]]".
+      iExists d, N'; iFrame.
+      iDestruct "eqs" as %[eqN eqD].
+      iPureIntro; split; auto.
+      eapply overlap_mono.
+      2-4: done.
+      clear -subA; red.
+      intro ξ.
+      rewrite /not_new !elem_of_difference !elem_of_of_gset.
+      set_solver.
+    Qed.
+
+    (** Closure: variables. *)
+    Lemma to_of_val v: to_val (of_val v) = Some v.
+    Proof.
+      destruct v; first done.
+      rewrite /= decide_left; done.
+    Qed.
+    
+    Lemma closed_variable (x: string) τ:
+      delayed_typed (<[x:=τ]>∅) hemp x x ∅ τ hemp.
+    Proof.
+      iIntros (D N σ) "[[env_names env] _]".
+      iDestruct "env_names" as %[domσ domD].
+      assert (is_Some (σ !! x)) as [v val_x].
+      { apply domσ; rewrite lookup_insert; eauto. }
+      assert (is_Some (D !! var x)) as [d conn_x].
+      { apply domD; rewrite lookup_insert; eauto. }
+      rewrite /= lookup_fmap val_x /=.
+      iApply wp_value'.
+      iExists N, (<[RET:=d]>D), d.
+      rewrite /int_i_emp; iFrame.
+      iSplit.
+      { rewrite lookup_insert; auto. }
+      iSplitL "env".
+      { iApply ("env" $! x τ v d).
+        iPureIntro; split; auto.
+        apply lookup_insert. }
+      iSplit; auto.
+      iAlways.
+      iIntros (N' σ' p K) "ctx [[env_names env] heap] move".
+      iDestruct "env_names" as %[domσ' _].
+      assert (is_Some (σ' !! x)) as [v' val'_x].
+      { apply domσ'; rewrite lookup_insert; eauto. }
+      rewrite /= lookup_fmap val'_x /=.
+      iModIntro; iExists v'; iFrame.
+      iExists d, N'.
+      rewrite lookup_insert.
+      iSplit; auto.
+      iSplitL "env".
+      - iApply ("env" $! x τ v' d).
+        rewrite lookup_insert; auto.
+      - by iExists 0.
+    Qed.
+
+    (** Closure: constants. *)
+    Lemma closed_true: delayed_typed ∅ hemp Ctrue Ctrue ∅ tbool hemp.
+    Proof.
+      iIntros (D N σ) "_".
+      change (Const Ctrue) with (of_val (VConst Ctrue)).
+      rewrite subst_closed_empty; last by apply val_closed.
+      iApply wp_value'.
+      iExists N, (<[RET:=VConst Ctrue]>D), (VConst Ctrue).
+      rewrite lookup_insert; iSplit; auto.
+      iSplit.
+      { iPureIntro; auto. }
+      iSplit; auto.
+      iAlways.
+      iIntros (N' σ' p K) "ctx _ move".
+      iModIntro.
+      iExists Ctrue.
+      rewrite subst_val; iFrame.
+      iExists Ctrue, N'.
+      rewrite lookup_insert; iSplit; auto.
+      iSplit.
+      - iPureIntro; auto.
+      - by iExists 0.
+    Qed.
+
+    Lemma closed_false: delayed_typed ∅ hemp Cfalse Cfalse ∅ tbool hemp.
+    Proof.
+      iIntros (D N σ) "_".
+      change (Const Cfalse) with (of_val (VConst Cfalse)).
+      rewrite subst_closed_empty; last by apply val_closed.
+      iApply wp_value'.
+      iExists N, (<[RET:=VConst Cfalse]>D), (VConst Cfalse).
+      rewrite lookup_insert; iSplit; auto.
+      iSplit.
+      { iPureIntro; auto. }
+      iSplit; auto.
+      iAlways.
+      iIntros (N' σ' p K) "ctx _ move".
+      iModIntro.
+      iExists Cfalse.
+      rewrite subst_val; iFrame.
+      iExists Cfalse, N'.
+      rewrite lookup_insert; iSplit; auto.
+      iSplit.
+      - iPureIntro; auto.
+      - by iExists 0.
+    Qed.
+
+    Lemma closed_unit: delayed_typed ∅ hemp Cunit Cunit ∅ tunit hemp.
+    Proof.
+      iIntros (D N σ) "_".
+      change (Const Cunit) with (of_val (VConst Cunit)).
+      rewrite subst_closed_empty; last by apply val_closed.
+      iApply wp_value'.
+      iExists N, (<[RET:=VConst Cunit]>D), (VConst Cunit).
+      rewrite lookup_insert; iSplit; auto.
+      iSplit.
+      { iPureIntro; auto. }
+      iSplit; auto.
+      iAlways.
+      iIntros (N' σ' p K) "ctx _ move".
+      iModIntro.
+      iExists Cunit.
+      rewrite subst_val; iFrame.
+      iExists Cunit, N'.
+      rewrite lookup_insert; iSplit; auto.
+      iSplit.
+      - iPureIntro; auto.
+      - by iExists 0.
+    Qed.
+
+    (** Closure: Memory operations *)
+    Lemma closed_alloc (x: string) (τ: type) ξ (ξ_fresh: ξ ∉ names τ):
+      delayed_typed (<[x:=τ]>∅) hemp (Alloc x) (Alloc x) {[ξ]} (tref ξ) (hpt ξ τ).
+    Proof.
+      iIntros (D N σ) "[[env_names env] _]".
+      iDestruct "env_names" as %[domσ domD].
+      assert (is_Some (σ !! x)) as [v val_x].
+      { apply domσ; rewrite lookup_insert; eauto. }
+      assert (is_Some (D !! var x)) as [d conn_x].
+      { apply domD; rewrite lookup_insert; eauto. }
+      rewrite /= lookup_fmap val_x /=.
+      iApply (wp_wand with "[]").
+      { iApply wp_alloc.
+        apply to_of_val. }
+      iIntros (?) "post".
+      iDestruct "post" as (l) "[% mt]"; subst.
+      iExists (<[ξ:=Loc l]>N), (<[RET := d]>(<[name ξ := d]>D)), d.
+      iSplit.
+      { iPureIntro.
+        rewrite lookup_insert; split; auto.
+        intro n.
+        rewrite /not_new elem_of_difference elem_of_of_gset not_elem_of_singleton => [[_ neqξ]].
+        rewrite lookup_insert_ne; congruence. }
+      iSplit.
+      { iPureIntro; exists l; rewrite lookup_insert; auto. }
+      iSplitL "mt env".
+      { iExists l, d, v; iFrame.
+        rewrite !lookup_insert lookup_insert_ne ?lookup_insert; last discriminate.
+        iSplit; auto.
+        iApply int_i_type_local.
+        4: iApply "env".
+        1,3: done.
+        - intros ξ' inξ'.
+          apply lookup_insert_ne.
+          congruence.
+        - iPureIntro.
+          split; first apply lookup_insert.
+          auto. }
+      iAlways.
+      iIntros (N' σ' p K) "ctx [[env_names env] _] move".
+      iDestruct "env_names" as %[domσ' _].
+      assert (is_Some (σ' !! x)) as [v' val'_x].
+      { apply domσ'; rewrite lookup_insert; eauto. }
+      rewrite /= lookup_fmap val'_x /=.
+      iMod (simulate_alloc with "ctx move") as (l') "[move post]"; eauto using to_of_val.
+      iModIntro; iExists (Cloc l'); iFrame.
+      iExists d, (<[ξ:=Loc l']>N').
+      iSplit.
+      { rewrite lookup_insert; iPureIntro; split; auto.
+        intros ξ'.
+        rewrite /not_new elem_of_difference elem_of_of_gset not_elem_of_singleton.
+        intros [_ neqξ].
+        rewrite lookup_insert_ne; done. }
+      iSplitR.
+      { iExists l'; rewrite lookup_insert; auto. }
+      iExists 0; cbn.
+      iExists l', d, v'; iFrame.
+      rewrite lookup_insert lookup_insert_ne ?lookup_insert; last discriminate.
+      iSplit; auto.
+      iSpecialize ("env" $! x τ v' d with "[]").
+      { rewrite lookup_insert; auto. }
+      iApply (int_s_type_local with "env"); auto.
+      intros ξ' inξ'.
+      rewrite lookup_insert_ne; congruence.
+    Qed.
+
+    Implicit Types x y: string.
+
+    Lemma int_s_heap_pt ξ τ D N:
+      int_s_heap (hpt ξ τ) D N ⊣⊢ int_s_heap_rec 0 (hpt ξ τ) D N.
+    Proof.
+      iSplit.
+      - iIntros "pre".
+        iDestruct "pre" as ([|n]) "pre"; auto.
+      - iIntros "pre".
+        iExists 0; done.
+    Qed.
+    
+    Lemma closed_read x ξ τ:
+      delayed_typed (<[x:=tref ξ]>∅) (hpt ξ τ) (Read x) (Read x) ∅ τ (hpt ξ τ).
+    Proof.
+      iIntros (D N σ) "[[env_names env] pt]".
+      iDestruct "env_names" as %[domσ domD].
+      assert (is_Some (σ !! x)) as [v val_x].
+      { apply domσ; rewrite lookup_insert; eauto. }
+      assert (is_Some (D !! var x)) as [d conn_x].
+      { apply domD; rewrite lookup_insert; eauto. }
+      rewrite /= lookup_fmap val_x /=.
+      iDestruct ("env" $! x (tref ξ) v d with "[]") as %[l [ref ->]].
+      { rewrite lookup_insert; auto. }
+      iDestruct "pt" as (l' d' v') "[eqs [mt #val]]".
+      iDestruct "eqs" as %[ref' eqd].
+      rewrite ref in ref'; injection ref' as <-.
+      iApply (wp_wand with "[mt]").
+      { iApply (wp_read with "mt"). }
+      iIntros (v) "[% mt]"; subst v'.
+      iExists N, (<[RET:=d']>D), d'.
+      iFrame.
+      rewrite lookup_insert.
+      iSplit; auto.
+      iSplit; auto.
+      iSplitL.
+      { iExists l, d', v; iFrame; iSplit; auto.
+        rewrite lookup_insert_ne; auto. }
+      iClear "val".
+      clear v l val_x ref N domσ σ.
+      iAlways.
+      iIntros (N σ p K) "ctx [[env_names env] pt] move".
+      iDestruct "env_names" as %[domσ _].
+      assert (is_Some (σ !! x)) as [v val_x].
+      { apply domσ; rewrite lookup_insert; eauto. }
+      rewrite /= lookup_fmap val_x /=.
+      iDestruct ("env" $! x (tref ξ) v d with "[]") as "ref".
+      { rewrite lookup_insert; auto. }
+      iDestruct "ref" as %[l [ref ->]].
+      rewrite int_s_heap_pt.
+      iDestruct "pt" as (l' d'' v) "[eqs [pt #type]]".
+      iDestruct "eqs" as %[eql eqd'].
+      rewrite ref in eql; injection eql as <-.
+      rewrite eqd in eqd'; injection eqd' as <-.
+      iMod (simulate_read with "ctx move pt") as "[move pt]"; auto.
+      iModIntro.
+      iExists v; iFrame.
+      iExists d', N.
+      rewrite lookup_insert.
+      iSplit; first done.
+      iSplit; first done.
+      rewrite int_s_heap_pt.
+      iExists l, d', v; iFrame; iSplit; auto.
+      rewrite lookup_insert_ne; auto.
+    Qed.
+
+    Lemma closed_write x y ξ τ (neq: x ≠ y):
+      delayed_typed (<[x:=tref ξ]>(<[y:=τ]>∅)) (hpt ξ τ) (Write x y) (Write x y) ∅ tunit (hpt ξ τ).
+    Proof.
+      iIntros (D N σ) "[[env_names #env] pt]".
+      iDestruct "env_names" as %[domσ domD].
+      assert (is_Some (σ !! x)) as [v val_x].
+      { apply domσ; rewrite lookup_insert; eauto. }
+      assert (is_Some (D !! var x)) as [d conn_x].
+      { apply domD; rewrite lookup_insert; eauto. }
+      rewrite /= lookup_fmap val_x /=.
+      assert (is_Some (σ !! y)) as [w val_y].
+      { apply domσ; rewrite lookup_insert_ne ?lookup_insert; eauto. }
+      assert (is_Some (D !! var y)) as [d' conn_y].
+      { apply domD; rewrite lookup_insert_ne ?lookup_insert; eauto. }
+      rewrite /= lookup_fmap val_y /=.
+      iDestruct "pt" as (l' dl v') "[eqs [mt #val]]".
+      iDestruct "eqs" as %[ref' eqd].
+      iDestruct ("env" $! x (tref ξ) v d with "[]") as %[l [ref ->]].
+      { rewrite lookup_insert; auto. }
+      rewrite ref in ref'; injection ref' as <-.
+      iPoseProof (wp_write ⊤ l (of_val w) w with "[mt]") as "wp".
+      { apply to_of_val. }
+      { iExists v'; iFrame. }
+      iApply (wp_wand with "wp").
+      iIntros (?) "[% mt]"; subst.
+      iExists N, (<[RET:=VConst Cunit]>(<[name ξ := d']>D)), Cunit.
+      rewrite lookup_insert.
+      iSplit; auto.
+      iSplit; auto.
+      iSplitL "mt".
+      { iExists l, d', w.
+        iFrame.
+        rewrite lookup_insert_ne ?lookup_insert; last auto.
+        iSplit; auto.
+        iApply ("env" $! y τ w d').
+        rewrite lookup_insert_ne; last done.
+        rewrite lookup_insert; auto. }
+      iClear "env".
+      iAlways.
+      iIntros (N' σ' p K) "ctx [[env_names #env] pt] move".
+      iDestruct "env_names" as %[domσ' _].
+      assert (is_Some (σ' !! x)) as [u val'_x].
+      { apply domσ'; rewrite lookup_insert; eauto. }
+      rewrite /= lookup_fmap val'_x /=.
+      assert (is_Some (σ' !! y)) as [w' val'_y].
+      { apply domσ'; rewrite lookup_insert_ne ?lookup_insert; eauto. }
+      rewrite lookup_fmap val'_y /=.
+      iDestruct ("env" $! x (tref ξ) u d with "[]") as %[l' [ref' ->]].
+      { rewrite lookup_insert; auto. }
+      rewrite int_s_heap_pt /= /int_s_pt.
+      iDestruct "pt" as (l'' d'' u') "[eqs [pt _]]".
+      iDestruct "eqs" as %[eql'' eqd''].
+      rewrite ref' in eql''; injection eql'' as <-.
+      rewrite eqd in eqd''; injection eqd'' as <-.
+      iMod (simulate_write with "ctx move [pt]") as "[move pt]".
+      1,2: eauto using to_of_val.
+      { iExists u'; iFrame. }
+      iModIntro; iExists Cunit; iFrame.
+      iExists Cunit, N'.
+      rewrite lookup_insert.
+      iSplit; auto.
+      iSplit; first done.
+      rewrite int_s_heap_pt.
+      iExists l', d', w'; iFrame.
+      rewrite lookup_insert_ne ?lookup_insert; last done.
+      iSplit; first done.
+      iApply ("env" $! y).
+      rewrite lookup_insert_ne ?lookup_insert; last done.
+      auto.
+    Qed.
+    
+    (** Closure: If *)
+    Lemma closed_if x Γ η A τ η' e₁ e₁' e₂ e₂' (x_type: Γ !! x = Some tbool):
+      delayed_typed Γ η e₁ e₁' A τ η' -∗
+                    delayed_typed Γ η e₂ e₂' A τ η' -∗
+                    delayed_typed Γ η (If x e₁ e₂) (If x e₁' e₂') A τ η'.
+    Proof.
+      iIntros "dtt dtf".
+      iIntros (D N σ) "[#env pre]".
+      iPoseProof ("env") as "[env_names env_types]".
+      iDestruct "env_names" as %[domσ domD].
+      assert (is_Some (σ !! x)) as [v val_x].
+      { apply domσ; rewrite x_type; eauto. }
+      assert (is_Some (D !! var x)) as [d conn_x].
+      { apply domD; rewrite x_type; eauto. }
+      rewrite /= lookup_fmap val_x /=.
+      iDestruct ("env_types" $! x tbool v d with "[]") as %[[->| ->] <-]; first auto.
+      { iApply wp_if_true.
+        iSpecialize ("dtt" $! D N σ with "[$env $pre]").
+        iApply (wp_wand with "dtt").
+        iClear "env env_types dtf".
+        iIntros (v) "post".
+        iDestruct "post" as (N' D' d') "[names [ty [heap #sim]]]".
+        iExists N', D', d'; iFrame.
+        clear N N' d' domσ σ val_x v.
+        iAlways.
+        iIntros (N σ p K) "#ctx [#env pre] move".
+        iPoseProof ("env") as "[env_names env_types]".
+        iDestruct "env_names" as %[domσ _].
+        assert (is_Some (σ !! x)) as [v val_x].
+        { apply domσ; rewrite x_type; eauto. }
+        iDestruct ("env_types" $! x tbool v Ctrue with "[]") as %[_ ->]; first auto.
+        rewrite /= lookup_fmap val_x /=.
+        iMod (simulate_if_true with "ctx move") as "move"; first auto.
+        iApply ("sim" with "ctx [$env $pre] move").
+      }{
+        iApply wp_if_false.
+        iSpecialize ("dtf" $! D N σ with "[$env $pre]").
+        iApply (wp_wand with "dtf").
+        iClear "env env_types dtt".
+        iIntros (v) "post".
+        iDestruct "post" as (N' D' d') "[names [ty [heap #sim]]]".
+        iExists N', D', d'; iFrame.
+        clear N N' d' domσ σ val_x v.
+        iAlways.
+        iIntros (N σ p K) "#ctx [#env pre] move".
+        iPoseProof ("env") as "[env_names env_types]".
+        iDestruct "env_names" as %[domσ _].
+        assert (is_Some (σ !! x)) as [v val_x].
+        { apply domσ; rewrite x_type; eauto. }
+        iDestruct ("env_types" $! x tbool v Cfalse with "[]") as %[_ ->]; first auto.
+        rewrite /= lookup_fmap val_x /=.
+        iMod (simulate_if_false with "ctx move") as "move"; first auto.
+        iApply ("sim" with "ctx [$env $pre] move").
+      }
+    Qed.
+
+    (** Closure: Let *)
+    Lemma closed_let x y Γ η A τ τ' η' e e' (x_type: Γ !! x = Some τ) (y_fresh: Γ !! y = None):
+      delayed_typed (<[y:= τ]> Γ) η e e' A τ' η' -∗
+                    delayed_typed Γ η (Let (BNamed y) x e) (Let (BNamed y) x e') A τ' η'.
+    Proof.
+      iIntros "del".
+      iIntros (D N σ) "[#env pre]".
+      iPoseProof ("env") as "[env_names env_types]".
+      iDestruct "env_names" as %[domσ domD].
+      assert (is_Some (σ !! x)) as [v val_x].
+      { apply domσ; rewrite x_type; eauto. }
+      assert (is_Some (D !! var x)) as [d conn_x].
+      { apply domD; rewrite x_type; eauto. }
+      rewrite /= lookup_fmap val_x /=.
+      iApply wp_app; first apply to_of_val.
+      rewrite /=.
+      rewrite subst_subst; cycle 1.
+      { intros x' e''.
+        rewrite lookup_delete_Some lookup_fmap fmap_Some => [[_ [v' [_ ->]]]].
+        apply val_closed. }
+      replace (subst_merge (<[y:=of_val v]> ∅) (delete y (of_val <$> σ)))
+        with (of_val <$> <[y:=v]>σ); cycle 1.
+      { apply map_eq; intro z.
+        rewrite /subst_merge lookup_merge /subst_merge'.
+        destruct (decide (y=z)) as [<-|neq].
+        - by rewrite lookup_delete lookup_fmap !lookup_insert.
+        - rewrite lookup_fmap !lookup_delete_ne; last done.
+          rewrite !lookup_insert_ne; auto.
+          rewrite lookup_empty lookup_fmap.
+          destruct (σ !! z) as [w|]; cbn; trivial.
+          rewrite subst_val; trivial. }
+      iSpecialize ("del" $! (<[var y := d]>D) N (<[y:=v]> σ) with "[env pre]").
+      { iSplit; first iSplit.
+        - iPureIntro.
+          setoid_rewrite lookup_insert_is_Some.
+          split; first by setoid_rewrite domσ.
+          intros z [eqy|[??]]; subst; auto.
+          destruct (decide (var y = var z)); auto.
+        - iIntros (x' τ'' v' d' [mtτ [mtv mtd]]).
+          destruct (decide (y = x')) as [<-|neq].
+          + rewrite lookup_insert in mtd; injection mtd as <-.
+            rewrite lookup_insert in mtv; injection mtv as <-.
+            rewrite lookup_insert in mtτ; injection mtτ as <-.
+            iApply ("env_types" $! x); auto.
+          + rewrite lookup_insert_ne in mtd; last congruence.
+            rewrite lookup_insert_ne in mtv; last congruence.
+            rewrite lookup_insert_ne in mtτ; last congruence.
+            iApply ("env_types" $! x'); auto.
+        - iApply (int_i_heap_local with "pre"); last done.
+          intro n.
+          rewrite /names_heap elem_of_of_list elem_of_list_fmap.
+          intros [ξ [-> _]].
+          apply lookup_insert_ne; done. }
+      iApply (wp_wand with "del").
+      iIntros (w) "post".
+      iDestruct "post" as (N' D' d') "[eqs [ty [heap #sim]]]".
+      iExists N', D', d'; iFrame.
+      iClear "env env_types".
+      clear v val_x N' d' w σ domσ N.
+      iAlways.
+      iIntros (N σ p K) "#ctx [#env pre] move".
+      cbn -[difference].
+      iPoseProof ("env") as "[env_names env_types]".
+      iDestruct "env_names" as %[domσ _].
+      assert (is_Some (σ !! x)) as [v val_x].
+      { apply domσ; rewrite x_type; eauto. }
+      rewrite /= lookup_fmap val_x /=.
+      iMod (simulate_app with "ctx move") as "move"; eauto using to_of_val.
+      rewrite /= subst_subst; cycle 1.
+      { intros x' e''.
+        rewrite lookup_delete_Some lookup_fmap fmap_Some => [[_ [v' [_ ->]]]].
+        apply val_closed. }
+      replace (subst_merge (<[y:=of_val v]> ∅) (delete y (of_val <$> σ)))
+        with (of_val <$> <[y:=v]>σ); cycle 1.
+      { apply map_eq; intro z.
+        rewrite /subst_merge lookup_merge /subst_merge'.
+        destruct (decide (y=z)) as [<-|neq].
+        - by rewrite lookup_delete lookup_fmap !lookup_insert.
+        - rewrite lookup_fmap !lookup_delete_ne; last done.
+          rewrite !lookup_insert_ne; auto.
+          rewrite lookup_empty lookup_fmap.
+          destruct (σ !! z) as [w|]; cbn; trivial.
+          rewrite subst_val; trivial. }
+      iSpecialize ("sim" $! N (<[y:=v]> σ) with "ctx [env pre]").
+      { iSplit; first iSplit.
+        - iPureIntro.
+          setoid_rewrite lookup_insert_is_Some.
+          split; first by setoid_rewrite domσ.
+          intros z [eqy|[??]]; subst; auto.
+          destruct (decide (var y = var z)); auto.
+        - iIntros (x' τ'' v' d' [mtτ [mtv mtd]]).
+          destruct (decide (y = x')) as [<-|neq].
+          + rewrite lookup_insert in mtd; injection mtd as <-.
+            rewrite lookup_insert in mtv; injection mtv as <-.
+            rewrite lookup_insert in mtτ; injection mtτ as <-.
+            iApply ("env_types" $! x); auto.
+          + rewrite lookup_insert_ne in mtd; last congruence.
+            rewrite lookup_insert_ne in mtv; last congruence.
+            rewrite lookup_insert_ne in mtτ; last congruence.
+            iApply ("env_types" $! x'); auto.
+        - iApply (int_s_heap_local with "pre"); last done.
+          intro n.
+          rewrite /names_heap elem_of_of_list elem_of_list_fmap.
+          intros [ξ [-> _]].
+          apply lookup_insert_ne; done. }
+      iApply "sim"; auto.
+    Qed.
+
+    (** Closure: Async operations *)
+    Lemma delete_insert_eq {A} (ξ: gname) (a: A) (m: gmap gname A):
+      delete ξ m = delete ξ (<[ξ:=a]>m).
+    Proof.
+      apply map_eq; intro ξ'.
+      destruct (decide (ξ = ξ')) as [<-|neq].
+      - by rewrite !lookup_delete.
+      - by rewrite !lookup_delete_ne ?lookup_insert_ne.
+    Qed.
+    
+    Lemma closed_post (Γ: env) (η: heap) e e' A (τ: type) (η': heap) ξ
+          (ξ_fresh_Γ: ξ ∉ names Γ) (ξ_fresh_η: ξ ∉ names η) (ξ_fresh_A: ξ ∉ A)
+          (τ_A: names τ ⊆ A) (η'_A: names η' ⊆ A):
+      delayed_typed Γ η e e' A τ η' -∗
+                    delayed_typed Γ η (Post e) (Post e') {[ξ]} (ttask ξ A τ) (hwait ξ A η').
+    Proof.
+      iIntros "del".
+      iIntros (D N σ) "pre"; cbn [subst].
+      (* Allocate ghost state *)
+      iApply fupd_wp.
+      iMod (own_alloc (@unset conn_mapC)) as (γD) "ownD"; first done.
+      iMod (own_alloc (@unset name_mapC)) as (γN) "ownN"; first done.
+      set (T := TaskData e' Γ η η' A D γD γN).
+      iMod (own_alloc (to_agree T)) as (γ) "#ownγ"; first done.
+      iAssert (WP subst (of_val <$> σ) e {{ x,
+                                            int_i_promise_body int_s_type int_s_heap (delete ξ N) A τ
+                                                               (int_i_type τ) γ  x ∗
+                                                               int_i_wait_body γ η'
+                                                               (int_i_heap η') A (delete ξ N) }})
+        with "[ownD ownN del pre]"
+        as "wp".
+      { iSpecialize ("del" with "pre").
+        iApply wp_fupd.
+        iApply (wp_wand with "del").
+        iIntros (v) "H".
+        iDestruct "H" as (N' D' d') "[eqs [ty [heap sim]]]".
+        iMod (own_update _ _ (agreed D') with "ownD") as "#ownD"; first apply oneshot_update.
+        iMod (own_update _ _ (agreed (delete ξ N': name_mapC)) with "ownN") as "#ownN";
+          first apply oneshot_update.
+        iModIntro.
+        iDestruct "eqs" as %[eqN eqd].
+        iSplitR "heap".
+        - iExists T, D', (delete ξ N').
+          iSplit.
+          { by repeat iSplit. }
+          iFrame.          
+          iExists d'; iFrame.
+          iSplit.
+          + iPureIntro; split; auto.
+            apply overlap_cast.          
+            assert (delete ξ N' ≡[ not_new A ]≡ delete ξ N).
+            { intros ξ' inξ'%eqN.
+              destruct (decide (ξ = ξ')) as [<-|neq].
+              - by rewrite !lookup_delete.
+              - by rewrite !lookup_delete_ne. }
+            eapply overlap_mono.
+            2-4: done.
+            intro ξ'.
+            rewrite /not_new elem_of_of_gset !elem_of_difference elem_of_of_gset.
+            set_solver.
+          + iApply (int_i_type_local with "ty").
+            1,3: done.
+            intros ξ' inξ'%τ_A.
+            apply lookup_delete_ne.
+            intros <-; contradiction.
+        - iExists T, D', (delete ξ N').
+          iFrame.
+          iSplit.
+          { by repeat iSplit. }
+          iSplit.
+          { iPureIntro.
+            apply overlap_cast.          
+            assert (delete ξ N' ≡[ not_new A ]≡ delete ξ N).
+            { intros ξ' inξ'%eqN.
+              destruct (decide (ξ = ξ')) as [<-|neq].
+              - by rewrite !lookup_delete.
+              - by rewrite !lookup_delete_ne. }
+            eapply overlap_mono.
+            2-4: done.
+            intro ξ'.
+            rewrite /not_new elem_of_of_gset !elem_of_difference elem_of_of_gset.
+            set_solver. }
+          iApply (int_i_heap_local with "heap"); first done.
+          intros ξ' inξ'%η'_A.
+          apply lookup_delete_ne.
+          intros <-; contradiction. }
+      iPoseProof (wp_post ⊤ with "wp") as "wp".
+      iModIntro.
+      iApply wp_fupd.
+      iApply (wp_wand with "wp").
+      iIntros (v) "H".
+      iDestruct "H" as (t) "[% wait]"; subst.
+      iPoseProof (wait_split with "wait") as "waits".
+      iPoseProof (fupd_mask_mono _ ⊤ with "waits") as "waits"; first auto.
+      iMod "waits" as "[promise wait]".      
+      iMod (inv_alloc promiseN with "promise") as "promise".
+      iAssert (int_i_type (Promise(ξ,A) τ) Cunit (<[ξ:=Task t γ]>N) (Ctid t))
+        with "[promise]" as "promise".
+      { cbn; iExists t, γ; iSplit.
+        - rewrite lookup_insert; auto.
+        - rewrite /typetranslation.wp_wait /=.
+          replace (delete ξ (<[ξ:=Task t γ]>N)) with (delete ξ N); first done.
+          apply map_eq; intro ξ'.
+          destruct (decide (ξ=ξ')) as [<-|neq].
+          + by rewrite !lookup_delete.
+          + rewrite !lookup_delete_ne ?lookup_insert_ne; auto. }
+      iAssert (int_i_heap (Wait(ξ,A) η') (<[name ξ:=VConst Cunit]>(<[RET:=VConst Cunit]>∅))
+                          (<[ξ:=Task t γ]>N))
+        with "[wait]" as "wait".
+      { cbn; iExists t, γ.
+        rewrite lookup_insert; iSplit; auto.
+        rewrite /typetranslation.wp_wait /=.
+        rewrite (delete_insert_eq ξ (Task t γ)); done. }
+      iModIntro.
+      iExists (<[ξ:=Task t γ]>N), (<[name ξ:=VConst Cunit]>(<[RET:=VConst Cunit]>∅)), (VConst Cunit).
+      iFrame.
+      iSplit.
+      { rewrite lookup_insert_ne; last discriminate.
+        rewrite lookup_insert.
+        iPureIntro; split; auto.
+        intro ξ'.
+        rewrite /not_new elem_of_difference elem_of_of_gset not_elem_of_singleton.
+        intros [_ ?].
+        rewrite lookup_insert_ne; done. }
+      clear σ N.
+      iAlways.
+      iIntros (N σ p K) "#ctx [env pre] move"; cbn -[difference].
+      iMod (simulate_post with "ctx move") as (p') "[move [move' neq]]"; auto.
+      iDestruct "pre" as (n) "pre".
+      iExists (Ctid p'); iFrame.
+      iExists (VConst Cunit), (<[ξ:=Task p' γ]>N).
+      iModIntro.
+      iAssert (int_s_heap (Wait(ξ,A) η') (<[name ξ:=VConst Cunit]>(<[RET:=VConst Cunit]>∅))
+                          (<[ξ:=Task p' γ]>N))
+        with "[pre move' env]" as "$".
+      { iExists (S n); cbn.
+        iExists p', γ, T, (<[ξ:=Task p' γ]>N), σ.
+        iSplit.
+        { iPureIntro; rewrite lookup_insert; repeat split; auto. }
+        iFrame.
+        iSplit.
+        - iApply (int_s_env_local with "env").
+          1,3: done.
+          intros ξ' inξ'.
+          apply lookup_insert_ne; congruence.
+        - iApply (int_s_heap_rec_local with "pre").
+          1,3: done.
+          intros ξ' inξ'.
+          apply lookup_insert_ne; congruence. }
+      iDestruct "neq" as %neq.
+      iPureIntro.
+      repeat split; auto.
+      - intros ξ'.
+        rewrite /not_new elem_of_difference elem_of_of_gset not_elem_of_singleton => [[_ ?]].
+        rewrite lookup_insert_ne; done.
+      - by rewrite lookup_insert_ne ?lookup_insert.
+      - exists p', γ.
+        rewrite lookup_insert; done.
+    Qed.
+
+    Instance wait_proper: Proper (eq ==> pointwise_relation _ (⊣⊢) ==> (⊣⊢)) (wait (Σ := Σ)).
+    Proof. solve_proper. Qed.
+    
+    Lemma closed_wait x ξ A (τ: type) (η: heap) (nssep: (↑waitN: coPset) ⊥ ↑promiseN)
+          (ξ_not_in_τ: ξ ∉ names τ) (ξ_not_in_η: ξ ∉ names η):
+      delayed_typed (<[x:=ttask ξ A τ]>∅) (hwait ξ A η) (Wait x) (Wait x) A τ η.
+    Proof.
+      iIntros (D N σ) "[[env_names env] pre]".
+      iDestruct "env_names" as %[domσ domD].
+      assert (is_Some (σ !! x)) as [v val_x].
+      { apply domσ; rewrite lookup_insert; eauto. }
+      assert (is_Some (D !! var x)) as [d conn_x].
+      { apply domD; rewrite lookup_insert; eauto. }
+      iDestruct ("env" $! x _ v d with "[]") as "#promise".
+      { rewrite lookup_insert; eauto. }
+      rewrite /= lookup_fmap val_x /=.
+      iDestruct "promise" as (t γ) "[eqs promise]".
+      iDestruct "eqs" as %[mtξ ->].
+      iApply fupd_wp.
+      iInv promiseN as "promisewait" "close".
+      rewrite /typetranslation.wp_wait /=.
+      iPoseProof (wait_split_later with "[promisewait]") as "split".
+      { iNext.
+        iApply (wait_proper with "promisewait"); first done.
+        iIntros (v); iSplit.
+        - iIntros "[pb _]"; iExact "pb".
+        - rewrite /int_i_promise_body.
+          iIntros "#pre".
+          iSplit; iExact "pre". }
+      iPoseProof (fupd_mask_mono _ (⊤ ∖ ↑promiseN) with "split") as "split"; first solve_ndisj.
+      iMod "split" as "[promisewait pw']".
+      iMod ("close" with "pw'") as "_".
+      iDestruct "pre" as (t' γ') "[mtξ' pre]".
+      rewrite mtξ; iDestruct "mtξ'" as %[=<- <-].
+      iPoseProof (wait_combine_later with "[$pre $promisewait]") as "wait".
+      iPoseProof (fupd_mask_mono _ ⊤ with "wait") as "wait"; first solve_ndisj.
+      iMod "wait" as "wait".
+      iModIntro.
+      iPoseProof (wp_wait with "wait") as "wp".
+      iApply (wp_wand with "wp").
+      iIntros (v) "[wb pb]".
+      iDestruct "wb" as (T D' N') "[[eqT [eqD eqN]] [eqnames heap]]".
+      iClear "promise".
+      iDestruct "pb" as (T' D'' N'') "[[eqT' [eqD' eqN']] [promise #sim]]".
+      iDestruct "promise" as (d') "[eqnames' type]".
+      iDestruct "eqnames" as %eqnames.
+      iDestruct "eqnames'" as %[eqD eqnames'].
+      iPoseProof (own_valid_2 with "eqT eqT'") as "eqT".
+      rewrite uPred.discrete_valid.
+      iDestruct "eqT" as %?%agree_op_invL'; subst T'.
+      iPoseProof (own_valid_2 with "eqD eqD'") as "eqD".
+      iPoseProof (own_valid_2 with "eqN eqN'") as "eqN".
+      rewrite !uPred.discrete_valid.
+      iDestruct "eqD" as %?%(agreed_valid D' D'')%leibniz_equiv; subst D''. 
+      iDestruct "eqN" as %?%(agreed_valid N' N'')%leibniz_equiv; subst N''.
+      iExists (N' ~[A]~> N).
+      iExists (<[RET:=d']>D').
+      iExists d'.      
+      iSplit.
+      { iPureIntro.
+        split; last by rewrite lookup_insert.
+        intros ξ'.
+        rewrite /not_new elem_of_difference elem_of_of_gset => [[_ notinξ]].
+        rewrite lookup_merge_along_not_in; done. }
+      iSplitL "type".
+      { iApply (int_i_type_local with "type").
+        1,3: done.
+        intros ξ' inξ'.
+        destruct (decide (ξ' ∈ A)) as [case|case].
+        - by rewrite lookup_merge_along_in.
+        - rewrite lookup_merge_along_not_in; last done.
+          rewrite (eqnames' ξ'); last set_solver.
+          rewrite lookup_delete_ne; first done.
+          congruence. }
+      iSplitL "heap".
+      { iApply (int_i_heap_local with "heap").
+        - intros n.
+          rewrite /names_heap elem_of_of_list elem_of_list_fmap.
+          intros [ξ' [-> inξ%elem_of_elements]].
+          apply lookup_insert_ne; done.
+        - intros ξ' inξ'.
+          destruct (decide (ξ' ∈ A)) as [case|case].
+          + by rewrite lookup_merge_along_in.
+          + rewrite lookup_merge_along_not_in; last done.
+            rewrite -(eqnames ξ'); last set_solver.
+            rewrite lookup_delete_ne; first done.
+            congruence. }
+      iAlways.
+      clear N N' mtξ eqnames eqnames' σ domσ val_x v.
+      iIntros (N σ p K) "#ctx [[env_names env] pre] move".
+      iDestruct "env_names" as %[domσ _].
+      assert (is_Some (σ !! x)) as [v val_x].
+      { apply domσ; rewrite lookup_insert; eauto. }
+      iSpecialize ("env" $! x _ v d with "[]").
+      { rewrite lookup_insert; auto. }
+      iDestruct "env" as %[t' [γ' [mtξ ->]]].
+      assert (γ' = γ) by admit. subst.
+      iDestruct "pre" as ([|n]) "pre".
+      { iDestruct "pre" as (t'' γ'' T' N'' D'') "[eqs [move' [_ []]]]". }
+      iDestruct "pre" as (t'' γ'' T' N'' D'') "[eqs [move' [env pre]]]".
+      rewrite /= lookup_fmap val_x /=.
+      iDestruct "eqs" as %[mtξ' [<- eqN]].
+      rewrite mtξ in mtξ'; injection mtξ' as <- <-.
+      iMod (simulate_wait_schedule with "ctx move move'") as "[move move']"; first done.
+      assert (T' = T) by admit. subst T'.
+      iMod ("sim" $! _ _ _ [] with "ctx [$env pre] move'") as (v) "[post move']".
+      { by iExists n. }
+      iDestruct "post" as (d'' N') "[eqnames [type heap]]".
+      iDestruct "eqnames" as %[eqN'' eqd''].
+      rewrite eqD in eqd''; injection eqd'' as <-.
+      iMod (simulate_done_schedule with "ctx move' move") as "[move' move]".
+      1,2: cbn; eauto using to_of_val.
+      iAssert (⌜t' ≠ p⌝) with "[move move']" as %neqp.
+      { iDestruct "move" as "[move _]".
+        iPoseProof (own_valid_2 with "move move'") as "valid".
+        rewrite /task_runnable /task_done -auth.auth_frag_op uPred.discrete_valid.
+        iDestruct "valid" as %valid; iPureIntro.
+        intros ->.
+        rewrite auth_valid_eq /= in valid.
+        specialize (valid p).
+        rewrite gmap.lookup_op !lookup_singleton in valid.
+        contradiction. }
+      iMod (simulate_wait_done with "ctx move move'") as "[move move']".
+      1,2: done.
+      iModIntro; iExists v; iFrame.
+      iExists d', (N' ~[A]~> N).
+      iSplit.
+      { iPureIntro.
+        split; last by rewrite lookup_insert.
+        intros ξ'.
+        rewrite /not_new elem_of_difference elem_of_of_gset => [[_ notinξ]].
+        rewrite lookup_merge_along_not_in; done. }
+      iSplitL "type".
+      { iApply (int_s_type_local with "type").
+        1,3: done.
+        intros ξ' inξ'.
+        destruct (decide (ξ' ∈ A)).
+        - by rewrite lookup_merge_along_in.
+        - rewrite lookup_merge_along_not_in; last done.
+          rewrite -(eqN'' ξ').
+          + rewrite (eqN ξ'); first done.
+            rewrite elem_of_
+          +
+    Qed.
+    
